coq/Syntax.v
@@ -1,16 +1,19 @@
 Require Export fintype.
 
+
+
+Section valtypecomptype.
 Inductive valtype  : Type :=
   | zero : valtype 
   | one : valtype 
-  | U : comptype  -> valtype 
-  | Sigma : valtype  -> valtype  -> valtype 
-  | cross : valtype  -> valtype  -> valtype 
+  | U : comptype   -> valtype 
+  | Sigma : valtype   -> valtype   -> valtype 
+  | cross : valtype   -> valtype   -> valtype 
  with comptype  : Type :=
   | cone : comptype 
-  | F : valtype  -> comptype 
-  | Pi : comptype  -> comptype  -> comptype 
-  | arrow : valtype  -> comptype  -> comptype .
+  | F : valtype   -> comptype 
+  | Pi : comptype   -> comptype   -> comptype 
+  | arrow : valtype   -> comptype   -> comptype .
 
 Lemma congr_zero  : zero  = zero  .
 Proof. congruence. Qed.
@@ -18,434 +21,449 @@ Proof. congruence. Qed.
 Lemma congr_one  : one  = one  .
 Proof. congruence. Qed.
 
-Lemma congr_U  { s0 : comptype  } { t0 : comptype  } : s0 = t0 -> U s0 = U t0 .
+Lemma congr_U  { s0 : comptype   } { t0 : comptype   } (H1 : s0 = t0) : U s0 = U t0 .
 Proof. congruence. Qed.
 
-Lemma congr_Sigma  { s0 : valtype  } { s1 : valtype  } { t0 : valtype  } { t1 : valtype  } : s0 = t0 -> s1 = t1 -> Sigma s0 s1 = Sigma t0 t1 .
+Lemma congr_Sigma  { s0 : valtype   } { s1 : valtype   } { t0 : valtype   } { t1 : valtype   } (H1 : s0 = t0) (H2 : s1 = t1) : Sigma s0 s1 = Sigma t0 t1 .
 Proof. congruence. Qed.
 
-Lemma congr_cross  { s0 : valtype  } { s1 : valtype  } { t0 : valtype  } { t1 : valtype  } : s0 = t0 -> s1 = t1 -> cross s0 s1 = cross t0 t1 .
+Lemma congr_cross  { s0 : valtype   } { s1 : valtype   } { t0 : valtype   } { t1 : valtype   } (H1 : s0 = t0) (H2 : s1 = t1) : cross s0 s1 = cross t0 t1 .
 Proof. congruence. Qed.
 
 Lemma congr_cone  : cone  = cone  .
 Proof. congruence. Qed.
 
-Lemma congr_F  { s0 : valtype  } { t0 : valtype  } : s0 = t0 -> F s0 = F t0 .
+Lemma congr_F  { s0 : valtype   } { t0 : valtype   } (H1 : s0 = t0) : F s0 = F t0 .
 Proof. congruence. Qed.
 
-Lemma congr_Pi  { s0 : comptype  } { s1 : comptype  } { t0 : comptype  } { t1 : comptype  } : s0 = t0 -> s1 = t1 -> Pi s0 s1 = Pi t0 t1 .
+Lemma congr_Pi  { s0 : comptype   } { s1 : comptype   } { t0 : comptype   } { t1 : comptype   } (H1 : s0 = t0) (H2 : s1 = t1) : Pi s0 s1 = Pi t0 t1 .
 Proof. congruence. Qed.
 
-Lemma congr_arrow  { s0 : valtype  } { s1 : comptype  } { t0 : valtype  } { t1 : comptype  } : s0 = t0 -> s1 = t1 -> arrow s0 s1 = arrow t0 t1 .
+Lemma congr_arrow  { s0 : valtype   } { s1 : comptype   } { t0 : valtype   } { t1 : comptype   } (H1 : s0 = t0) (H2 : s1 = t1) : arrow s0 s1 = arrow t0 t1 .
 Proof. congruence. Qed.
 
+End valtypecomptype.
+
+
+Section valuecomp.
 Inductive value (nvalue : nat) : Type :=
-  | var_value : fin (nvalue) -> value (nvalue)
+  | var_value : (fin) (nvalue) -> value (nvalue)
   | u : value (nvalue)
-  | pair : value (nvalue) -> value (nvalue) -> value (nvalue)
-  | inj : bool  -> value (nvalue) -> value (nvalue)
-  | thunk : comp (nvalue) -> value (nvalue)
+  | pair : value  (nvalue) -> value  (nvalue) -> value (nvalue)
+  | inj : bool   -> value  (nvalue) -> value (nvalue)
+  | thunk : comp  (nvalue) -> value (nvalue)
  with comp (nvalue : nat) : Type :=
   | cu : comp (nvalue)
-  | force : value (nvalue) -> comp (nvalue)
-  | lambda : comp (S nvalue) -> comp (nvalue)
-  | app : comp (nvalue) -> value (nvalue) -> comp (nvalue)
-  | tuple : comp (nvalue) -> comp (nvalue) -> comp (nvalue)
-  | ret : value (nvalue) -> comp (nvalue)
-  | letin : comp (nvalue) -> comp (S nvalue) -> comp (nvalue)
-  | proj : bool  -> comp (nvalue) -> comp (nvalue)
-  | caseZ : value (nvalue) -> comp (nvalue)
-  | caseS : value (nvalue) -> comp (S nvalue) -> comp (S nvalue) -> comp (nvalue)
-  | caseP : value (nvalue) -> comp (S (S nvalue)) -> comp (nvalue).
+  | force : value  (nvalue) -> comp (nvalue)
+  | lambda : comp  ((S) nvalue) -> comp (nvalue)
+  | app : comp  (nvalue) -> value  (nvalue) -> comp (nvalue)
+  | tuple : comp  (nvalue) -> comp  (nvalue) -> comp (nvalue)
+  | ret : value  (nvalue) -> comp (nvalue)
+  | letin : comp  (nvalue) -> comp  ((S) nvalue) -> comp (nvalue)
+  | proj : bool   -> comp  (nvalue) -> comp (nvalue)
+  | caseZ : value  (nvalue) -> comp (nvalue)
+  | caseS : value  (nvalue) -> comp  ((S) nvalue) -> comp  ((S) nvalue) -> comp (nvalue)
+  | caseP : value  (nvalue) -> comp  ((S) ((S) nvalue)) -> comp (nvalue).
 
 Lemma congr_u { mvalue : nat } : u (mvalue) = u (mvalue) .
 Proof. congruence. Qed.
 
-Lemma congr_pair { mvalue : nat } { s0 : value (mvalue) } { s1 : value (mvalue) } { t0 : value (mvalue) } { t1 : value (mvalue) } : s0 = t0 -> s1 = t1 -> pair (mvalue) s0 s1 = pair (mvalue) t0 t1 .
+Lemma congr_pair { mvalue : nat } { s0 : value  (mvalue) } { s1 : value  (mvalue) } { t0 : value  (mvalue) } { t1 : value  (mvalue) } (H1 : s0 = t0) (H2 : s1 = t1) : pair (mvalue) s0 s1 = pair (mvalue) t0 t1 .
 Proof. congruence. Qed.
 
-Lemma congr_inj { mvalue : nat } { s0 : bool  } { s1 : value (mvalue) } { t0 : bool  } { t1 : value (mvalue) } : s0 = t0 -> s1 = t1 -> inj (mvalue) s0 s1 = inj (mvalue) t0 t1 .
+Lemma congr_inj { mvalue : nat } { s0 : bool   } { s1 : value  (mvalue) } { t0 : bool   } { t1 : value  (mvalue) } (H1 : s0 = t0) (H2 : s1 = t1) : inj (mvalue) s0 s1 = inj (mvalue) t0 t1 .
 Proof. congruence. Qed.
 
-Lemma congr_thunk { mvalue : nat } { s0 : comp (mvalue) } { t0 : comp (mvalue) } : s0 = t0 -> thunk (mvalue) s0 = thunk (mvalue) t0 .
+Lemma congr_thunk { mvalue : nat } { s0 : comp  (mvalue) } { t0 : comp  (mvalue) } (H1 : s0 = t0) : thunk (mvalue) s0 = thunk (mvalue) t0 .
 Proof. congruence. Qed.
 
 Lemma congr_cu { mvalue : nat } : cu (mvalue) = cu (mvalue) .
 Proof. congruence. Qed.
 
-Lemma congr_force { mvalue : nat } { s0 : value (mvalue) } { t0 : value (mvalue) } : s0 = t0 -> force (mvalue) s0 = force (mvalue) t0 .
+Lemma congr_force { mvalue : nat } { s0 : value  (mvalue) } { t0 : value  (mvalue) } (H1 : s0 = t0) : force (mvalue) s0 = force (mvalue) t0 .
 Proof. congruence. Qed.
 
-Lemma congr_lambda { mvalue : nat } { s0 : comp (S mvalue) } { t0 : comp (S mvalue) } : s0 = t0 -> lambda (mvalue) s0 = lambda (mvalue) t0 .
+Lemma congr_lambda { mvalue : nat } { s0 : comp  ((S) mvalue) } { t0 : comp  ((S) mvalue) } (H1 : s0 = t0) : lambda (mvalue) s0 = lambda (mvalue) t0 .
 Proof. congruence. Qed.
 
-Lemma congr_app { mvalue : nat } { s0 : comp (mvalue) } { s1 : value (mvalue) } { t0 : comp (mvalue) } { t1 : value (mvalue) } : s0 = t0 -> s1 = t1 -> app (mvalue) s0 s1 = app (mvalue) t0 t1 .
+Lemma congr_app { mvalue : nat } { s0 : comp  (mvalue) } { s1 : value  (mvalue) } { t0 : comp  (mvalue) } { t1 : value  (mvalue) } (H1 : s0 = t0) (H2 : s1 = t1) : app (mvalue) s0 s1 = app (mvalue) t0 t1 .
 Proof. congruence. Qed.
 
-Lemma congr_tuple { mvalue : nat } { s0 : comp (mvalue) } { s1 : comp (mvalue) } { t0 : comp (mvalue) } { t1 : comp (mvalue) } : s0 = t0 -> s1 = t1 -> tuple (mvalue) s0 s1 = tuple (mvalue) t0 t1 .
+Lemma congr_tuple { mvalue : nat } { s0 : comp  (mvalue) } { s1 : comp  (mvalue) } { t0 : comp  (mvalue) } { t1 : comp  (mvalue) } (H1 : s0 = t0) (H2 : s1 = t1) : tuple (mvalue) s0 s1 = tuple (mvalue) t0 t1 .
 Proof. congruence. Qed.
 
-Lemma congr_ret { mvalue : nat } { s0 : value (mvalue) } { t0 : value (mvalue) } : s0 = t0 -> ret (mvalue) s0 = ret (mvalue) t0 .
+Lemma congr_ret { mvalue : nat } { s0 : value  (mvalue) } { t0 : value  (mvalue) } (H1 : s0 = t0) : ret (mvalue) s0 = ret (mvalue) t0 .
 Proof. congruence. Qed.
 
-Lemma congr_letin { mvalue : nat } { s0 : comp (mvalue) } { s1 : comp (S mvalue) } { t0 : comp (mvalue) } { t1 : comp (S mvalue) } : s0 = t0 -> s1 = t1 -> letin (mvalue) s0 s1 = letin (mvalue) t0 t1 .
+Lemma congr_letin { mvalue : nat } { s0 : comp  (mvalue) } { s1 : comp  ((S) mvalue) } { t0 : comp  (mvalue) } { t1 : comp  ((S) mvalue) } (H1 : s0 = t0) (H2 : s1 = t1) : letin (mvalue) s0 s1 = letin (mvalue) t0 t1 .
 Proof. congruence. Qed.
 
-Lemma congr_proj { mvalue : nat } { s0 : bool  } { s1 : comp (mvalue) } { t0 : bool  } { t1 : comp (mvalue) } : s0 = t0 -> s1 = t1 -> proj (mvalue) s0 s1 = proj (mvalue) t0 t1 .
+Lemma congr_proj { mvalue : nat } { s0 : bool   } { s1 : comp  (mvalue) } { t0 : bool   } { t1 : comp  (mvalue) } (H1 : s0 = t0) (H2 : s1 = t1) : proj (mvalue) s0 s1 = proj (mvalue) t0 t1 .
 Proof. congruence. Qed.
 
-Lemma congr_caseZ { mvalue : nat } { s0 : value (mvalue) } { t0 : value (mvalue) } : s0 = t0 -> caseZ (mvalue) s0 = caseZ (mvalue) t0 .
+Lemma congr_caseZ { mvalue : nat } { s0 : value  (mvalue) } { t0 : value  (mvalue) } (H1 : s0 = t0) : caseZ (mvalue) s0 = caseZ (mvalue) t0 .
 Proof. congruence. Qed.
 
-Lemma congr_caseS { mvalue : nat } { s0 : value (mvalue) } { s1 : comp (S mvalue) } { s2 : comp (S mvalue) } { t0 : value (mvalue) } { t1 : comp (S mvalue) } { t2 : comp (S mvalue) } : s0 = t0 -> s1 = t1 -> s2 = t2 -> caseS (mvalue) s0 s1 s2 = caseS (mvalue) t0 t1 t2 .
+Lemma congr_caseS { mvalue : nat } { s0 : value  (mvalue) } { s1 : comp  ((S) mvalue) } { s2 : comp  ((S) mvalue) } { t0 : value  (mvalue) } { t1 : comp  ((S) mvalue) } { t2 : comp  ((S) mvalue) } (H1 : s0 = t0) (H2 : s1 = t1) (H3 : s2 = t2) : caseS (mvalue) s0 s1 s2 = caseS (mvalue) t0 t1 t2 .
 Proof. congruence. Qed.
 
-Lemma congr_caseP { mvalue : nat } { s0 : value (mvalue) } { s1 : comp (S (S mvalue)) } { t0 : value (mvalue) } { t1 : comp (S (S mvalue)) } : s0 = t0 -> s1 = t1 -> caseP (mvalue) s0 s1 = caseP (mvalue) t0 t1 .
+Lemma congr_caseP { mvalue : nat } { s0 : value  (mvalue) } { s1 : comp  ((S) ((S) mvalue)) } { t0 : value  (mvalue) } { t1 : comp  ((S) ((S) mvalue)) } (H1 : s0 = t0) (H2 : s1 = t1) : caseP (mvalue) s0 s1 = caseP (mvalue) t0 t1 .
 Proof. congruence. Qed.
 
-Definition upRen_value_value { m : nat } { n : nat } (xi : fin (m) -> fin (n)) : _ :=
-  up_ren xi.
+Definition upRen_value_value { m : nat } { n : nat } (xi : (fin) (m) -> (fin) (n)) : (fin) ((S) (m)) -> (fin) ((S) (n)) :=
+  (up_ren) xi.
 
-Fixpoint ren_value { mvalue : nat } { nvalue : nat } (xivalue : fin (mvalue) -> fin (nvalue)) (s : value (mvalue)) : _ :=
-    match s with
+Fixpoint ren_value { mvalue : nat } { nvalue : nat } (xivalue : (fin) (mvalue) -> (fin) (nvalue)) (s : value (mvalue)) : value (nvalue) :=
+    match s return value (nvalue) with
     | var_value (_) s => (var_value (nvalue)) (xivalue s)
     | u (_)  => u (nvalue)
-    | pair (_) s0 s1 => pair (nvalue) (ren_value xivalue s0) (ren_value xivalue s1)
-    | inj (_) s0 s1 => inj (nvalue) s0 (ren_value xivalue s1)
-    | thunk (_) s0 => thunk (nvalue) (ren_comp xivalue s0)
+    | pair (_) s0 s1 => pair (nvalue) ((ren_value xivalue) s0) ((ren_value xivalue) s1)
+    | inj (_) s0 s1 => inj (nvalue) ((fun x => x) s0) ((ren_value xivalue) s1)
+    | thunk (_) s0 => thunk (nvalue) ((ren_comp xivalue) s0)
     end
- with ren_comp { mvalue : nat } { nvalue : nat } (xivalue : fin (mvalue) -> fin (nvalue)) (s : comp (mvalue)) : _ :=
-    match s with
+ with ren_comp { mvalue : nat } { nvalue : nat } (xivalue : (fin) (mvalue) -> (fin) (nvalue)) (s : comp (mvalue)) : comp (nvalue) :=
+    match s return comp (nvalue) with
     | cu (_)  => cu (nvalue)
-    | force (_) s0 => force (nvalue) (ren_value xivalue s0)
-    | lambda (_) s0 => lambda (nvalue) (ren_comp (upRen_value_value xivalue) s0)
-    | app (_) s0 s1 => app (nvalue) (ren_comp xivalue s0) (ren_value xivalue s1)
-    | tuple (_) s0 s1 => tuple (nvalue) (ren_comp xivalue s0) (ren_comp xivalue s1)
-    | ret (_) s0 => ret (nvalue) (ren_value xivalue s0)
-    | letin (_) s0 s1 => letin (nvalue) (ren_comp xivalue s0) (ren_comp (upRen_value_value xivalue) s1)
-    | proj (_) s0 s1 => proj (nvalue) s0 (ren_comp xivalue s1)
-    | caseZ (_) s0 => caseZ (nvalue) (ren_value xivalue s0)
-    | caseS (_) s0 s1 s2 => caseS (nvalue) (ren_value xivalue s0) (ren_comp (upRen_value_value xivalue) s1) (ren_comp (upRen_value_value xivalue) s2)
-    | caseP (_) s0 s1 => caseP (nvalue) (ren_value xivalue s0) (ren_comp (upRen_value_value (upRen_value_value xivalue)) s1)
+    | force (_) s0 => force (nvalue) ((ren_value xivalue) s0)
+    | lambda (_) s0 => lambda (nvalue) ((ren_comp (upRen_value_value xivalue)) s0)
+    | app (_) s0 s1 => app (nvalue) ((ren_comp xivalue) s0) ((ren_value xivalue) s1)
+    | tuple (_) s0 s1 => tuple (nvalue) ((ren_comp xivalue) s0) ((ren_comp xivalue) s1)
+    | ret (_) s0 => ret (nvalue) ((ren_value xivalue) s0)
+    | letin (_) s0 s1 => letin (nvalue) ((ren_comp xivalue) s0) ((ren_comp (upRen_value_value xivalue)) s1)
+    | proj (_) s0 s1 => proj (nvalue) ((fun x => x) s0) ((ren_comp xivalue) s1)
+    | caseZ (_) s0 => caseZ (nvalue) ((ren_value xivalue) s0)
+    | caseS (_) s0 s1 s2 => caseS (nvalue) ((ren_value xivalue) s0) ((ren_comp (upRen_value_value xivalue)) s1) ((ren_comp (upRen_value_value xivalue)) s2)
+    | caseP (_) s0 s1 => caseP (nvalue) ((ren_value xivalue) s0) ((ren_comp (upRen_value_value (upRen_value_value xivalue))) s1)
     end.
 
-Definition up_value_value { m : nat } { nvalue : nat } (sigma : fin (m) -> value (nvalue)) : _ :=
-  scons ((var_value (S nvalue)) var_zero) (funcomp (ren_value shift) sigma).
+Definition up_value_value { m : nat } { nvalue : nat } (sigma : (fin) (m) -> value (nvalue)) : (fin) ((S) (m)) -> value ((S) nvalue) :=
+  (scons) ((var_value ((S) nvalue)) (var_zero)) ((funcomp) (ren_value (shift)) sigma).
 
-Fixpoint subst_value { mvalue : nat } { nvalue : nat } (sigmavalue : fin (mvalue) -> value (nvalue)) (s : value (mvalue)) : _ :=
-    match s with
+Fixpoint subst_value { mvalue : nat } { nvalue : nat } (sigmavalue : (fin) (mvalue) -> value (nvalue)) (s : value (mvalue)) : value (nvalue) :=
+    match s return value (nvalue) with
     | var_value (_) s => sigmavalue s
     | u (_)  => u (nvalue)
-    | pair (_) s0 s1 => pair (nvalue) (subst_value sigmavalue s0) (subst_value sigmavalue s1)
-    | inj (_) s0 s1 => inj (nvalue) s0 (subst_value sigmavalue s1)
-    | thunk (_) s0 => thunk (nvalue) (subst_comp sigmavalue s0)
+    | pair (_) s0 s1 => pair (nvalue) ((subst_value sigmavalue) s0) ((subst_value sigmavalue) s1)
+    | inj (_) s0 s1 => inj (nvalue) ((fun x => x) s0) ((subst_value sigmavalue) s1)
+    | thunk (_) s0 => thunk (nvalue) ((subst_comp sigmavalue) s0)
     end
- with subst_comp { mvalue : nat } { nvalue : nat } (sigmavalue : fin (mvalue) -> value (nvalue)) (s : comp (mvalue)) : _ :=
-    match s with
+ with subst_comp { mvalue : nat } { nvalue : nat } (sigmavalue : (fin) (mvalue) -> value (nvalue)) (s : comp (mvalue)) : comp (nvalue) :=
+    match s return comp (nvalue) with
     | cu (_)  => cu (nvalue)
-    | force (_) s0 => force (nvalue) (subst_value sigmavalue s0)
-    | lambda (_) s0 => lambda (nvalue) (subst_comp (up_value_value sigmavalue) s0)
-    | app (_) s0 s1 => app (nvalue) (subst_comp sigmavalue s0) (subst_value sigmavalue s1)
-    | tuple (_) s0 s1 => tuple (nvalue) (subst_comp sigmavalue s0) (subst_comp sigmavalue s1)
-    | ret (_) s0 => ret (nvalue) (subst_value sigmavalue s0)
-    | letin (_) s0 s1 => letin (nvalue) (subst_comp sigmavalue s0) (subst_comp (up_value_value sigmavalue) s1)
-    | proj (_) s0 s1 => proj (nvalue) s0 (subst_comp sigmavalue s1)
-    | caseZ (_) s0 => caseZ (nvalue) (subst_value sigmavalue s0)
-    | caseS (_) s0 s1 s2 => caseS (nvalue) (subst_value sigmavalue s0) (subst_comp (up_value_value sigmavalue) s1) (subst_comp (up_value_value sigmavalue) s2)
-    | caseP (_) s0 s1 => caseP (nvalue) (subst_value sigmavalue s0) (subst_comp (up_value_value (up_value_value sigmavalue)) s1)
+    | force (_) s0 => force (nvalue) ((subst_value sigmavalue) s0)
+    | lambda (_) s0 => lambda (nvalue) ((subst_comp (up_value_value sigmavalue)) s0)
+    | app (_) s0 s1 => app (nvalue) ((subst_comp sigmavalue) s0) ((subst_value sigmavalue) s1)
+    | tuple (_) s0 s1 => tuple (nvalue) ((subst_comp sigmavalue) s0) ((subst_comp sigmavalue) s1)
+    | ret (_) s0 => ret (nvalue) ((subst_value sigmavalue) s0)
+    | letin (_) s0 s1 => letin (nvalue) ((subst_comp sigmavalue) s0) ((subst_comp (up_value_value sigmavalue)) s1)
+    | proj (_) s0 s1 => proj (nvalue) ((fun x => x) s0) ((subst_comp sigmavalue) s1)
+    | caseZ (_) s0 => caseZ (nvalue) ((subst_value sigmavalue) s0)
+    | caseS (_) s0 s1 s2 => caseS (nvalue) ((subst_value sigmavalue) s0) ((subst_comp (up_value_value sigmavalue)) s1) ((subst_comp (up_value_value sigmavalue)) s2)
+    | caseP (_) s0 s1 => caseP (nvalue) ((subst_value sigmavalue) s0) ((subst_comp (up_value_value (up_value_value sigmavalue))) s1)
     end.
 
-Definition upId_value_value { mvalue : nat } (sigma : fin (mvalue) -> value (mvalue)) (Eq : forall x, sigma x = (var_value (mvalue)) x) : forall x, (up_value_value sigma) x = (var_value (S mvalue)) x :=
+Definition upId_value_value { mvalue : nat } (sigma : (fin) (mvalue) -> value (mvalue)) (Eq : forall x, sigma x = (var_value (mvalue)) x) : forall x, (up_value_value sigma) x = (var_value ((S) mvalue)) x :=
   fun n => match n with
-  | Some n => ap (ren_value shift) (Eq n)
-  | None => eq_refl
+  | Some fin_n => (ap) (ren_value (shift)) (Eq fin_n)
+  | None  => eq_refl
   end.
 
-Fixpoint idSubst_value { mvalue : nat } (sigmavalue : fin (mvalue) -> value (mvalue)) (Eqvalue : forall x, sigmavalue x = (var_value (mvalue)) x) (s : value (mvalue)) : subst_value sigmavalue s = s :=
-    match s with
+Fixpoint idSubst_value { mvalue : nat } (sigmavalue : (fin) (mvalue) -> value (mvalue)) (Eqvalue : forall x, sigmavalue x = (var_value (mvalue)) x) (s : value (mvalue)) : subst_value sigmavalue s = s :=
+    match s return subst_value sigmavalue s = s with
     | var_value (_) s => Eqvalue s
     | u (_)  => congr_u 
-    | pair (_) s0 s1 => congr_pair (idSubst_value sigmavalue Eqvalue s0) (idSubst_value sigmavalue Eqvalue s1)
-    | inj (_) s0 s1 => congr_inj (eq_refl s0) (idSubst_value sigmavalue Eqvalue s1)
-    | thunk (_) s0 => congr_thunk (idSubst_comp sigmavalue Eqvalue s0)
+    | pair (_) s0 s1 => congr_pair ((idSubst_value sigmavalue Eqvalue) s0) ((idSubst_value sigmavalue Eqvalue) s1)
+    | inj (_) s0 s1 => congr_inj ((fun x => (eq_refl) x) s0) ((idSubst_value sigmavalue Eqvalue) s1)
+    | thunk (_) s0 => congr_thunk ((idSubst_comp sigmavalue Eqvalue) s0)
     end
- with idSubst_comp { mvalue : nat } (sigmavalue : fin (mvalue) -> value (mvalue)) (Eqvalue : forall x, sigmavalue x = (var_value (mvalue)) x) (s : comp (mvalue)) : subst_comp sigmavalue s = s :=
-    match s with
+ with idSubst_comp { mvalue : nat } (sigmavalue : (fin) (mvalue) -> value (mvalue)) (Eqvalue : forall x, sigmavalue x = (var_value (mvalue)) x) (s : comp (mvalue)) : subst_comp sigmavalue s = s :=
+    match s return subst_comp sigmavalue s = s with
     | cu (_)  => congr_cu 
-    | force (_) s0 => congr_force (idSubst_value sigmavalue Eqvalue s0)
-    | lambda (_) s0 => congr_lambda (idSubst_comp (up_value_value sigmavalue) (upId_value_value (_) Eqvalue) s0)
-    | app (_) s0 s1 => congr_app (idSubst_comp sigmavalue Eqvalue s0) (idSubst_value sigmavalue Eqvalue s1)
-    | tuple (_) s0 s1 => congr_tuple (idSubst_comp sigmavalue Eqvalue s0) (idSubst_comp sigmavalue Eqvalue s1)
-    | ret (_) s0 => congr_ret (idSubst_value sigmavalue Eqvalue s0)
-    | letin (_) s0 s1 => congr_letin (idSubst_comp sigmavalue Eqvalue s0) (idSubst_comp (up_value_value sigmavalue) (upId_value_value (_) Eqvalue) s1)
-    | proj (_) s0 s1 => congr_proj (eq_refl s0) (idSubst_comp sigmavalue Eqvalue s1)
-    | caseZ (_) s0 => congr_caseZ (idSubst_value sigmavalue Eqvalue s0)
-    | caseS (_) s0 s1 s2 => congr_caseS (idSubst_value sigmavalue Eqvalue s0) (idSubst_comp (up_value_value sigmavalue) (upId_value_value (_) Eqvalue) s1) (idSubst_comp (up_value_value sigmavalue) (upId_value_value (_) Eqvalue) s2)
-    | caseP (_) s0 s1 => congr_caseP (idSubst_value sigmavalue Eqvalue s0) (idSubst_comp (up_value_value (up_value_value sigmavalue)) (upId_value_value (_) (upId_value_value (_) Eqvalue)) s1)
+    | force (_) s0 => congr_force ((idSubst_value sigmavalue Eqvalue) s0)
+    | lambda (_) s0 => congr_lambda ((idSubst_comp (up_value_value sigmavalue) (upId_value_value (_) Eqvalue)) s0)
+    | app (_) s0 s1 => congr_app ((idSubst_comp sigmavalue Eqvalue) s0) ((idSubst_value sigmavalue Eqvalue) s1)
+    | tuple (_) s0 s1 => congr_tuple ((idSubst_comp sigmavalue Eqvalue) s0) ((idSubst_comp sigmavalue Eqvalue) s1)
+    | ret (_) s0 => congr_ret ((idSubst_value sigmavalue Eqvalue) s0)
+    | letin (_) s0 s1 => congr_letin ((idSubst_comp sigmavalue Eqvalue) s0) ((idSubst_comp (up_value_value sigmavalue) (upId_value_value (_) Eqvalue)) s1)
+    | proj (_) s0 s1 => congr_proj ((fun x => (eq_refl) x) s0) ((idSubst_comp sigmavalue Eqvalue) s1)
+    | caseZ (_) s0 => congr_caseZ ((idSubst_value sigmavalue Eqvalue) s0)
+    | caseS (_) s0 s1 s2 => congr_caseS ((idSubst_value sigmavalue Eqvalue) s0) ((idSubst_comp (up_value_value sigmavalue) (upId_value_value (_) Eqvalue)) s1) ((idSubst_comp (up_value_value sigmavalue) (upId_value_value (_) Eqvalue)) s2)
+    | caseP (_) s0 s1 => congr_caseP ((idSubst_value sigmavalue Eqvalue) s0) ((idSubst_comp (up_value_value (up_value_value sigmavalue)) (upId_value_value (_) (upId_value_value (_) Eqvalue))) s1)
     end.
 
-Definition upExtRen_value_value { m : nat } { n : nat } (xi : fin (m) -> fin (n)) (zeta : fin (m) -> fin (n)) (Eq : forall x, xi x = zeta x) : forall x, (upRen_value_value xi) x = (upRen_value_value zeta) x :=
+Definition upExtRen_value_value { m : nat } { n : nat } (xi : (fin) (m) -> (fin) (n)) (zeta : (fin) (m) -> (fin) (n)) (Eq : forall x, xi x = zeta x) : forall x, (upRen_value_value xi) x = (upRen_value_value zeta) x :=
   fun n => match n with
-  | Some n => ap shift (Eq n)
-  | None => eq_refl
+  | Some fin_n => (ap) (shift) (Eq fin_n)
+  | None  => eq_refl
   end.
 
-Fixpoint extRen_value { mvalue : nat } { nvalue : nat } (xivalue : fin (mvalue) -> fin (nvalue)) (zetavalue : fin (mvalue) -> fin (nvalue)) (Eqvalue : forall x, xivalue x = zetavalue x) (s : value (mvalue)) : ren_value xivalue s = ren_value zetavalue s :=
-    match s with
-    | var_value (_) s => ap (var_value (nvalue)) (Eqvalue s)
+Fixpoint extRen_value { mvalue : nat } { nvalue : nat } (xivalue : (fin) (mvalue) -> (fin) (nvalue)) (zetavalue : (fin) (mvalue) -> (fin) (nvalue)) (Eqvalue : forall x, xivalue x = zetavalue x) (s : value (mvalue)) : ren_value xivalue s = ren_value zetavalue s :=
+    match s return ren_value xivalue s = ren_value zetavalue s with
+    | var_value (_) s => (ap) (var_value (nvalue)) (Eqvalue s)
     | u (_)  => congr_u 
-    | pair (_) s0 s1 => congr_pair (extRen_value xivalue zetavalue Eqvalue s0) (extRen_value xivalue zetavalue Eqvalue s1)
-    | inj (_) s0 s1 => congr_inj (eq_refl s0) (extRen_value xivalue zetavalue Eqvalue s1)
-    | thunk (_) s0 => congr_thunk (extRen_comp xivalue zetavalue Eqvalue s0)
+    | pair (_) s0 s1 => congr_pair ((extRen_value xivalue zetavalue Eqvalue) s0) ((extRen_value xivalue zetavalue Eqvalue) s1)
+    | inj (_) s0 s1 => congr_inj ((fun x => (eq_refl) x) s0) ((extRen_value xivalue zetavalue Eqvalue) s1)
+    | thunk (_) s0 => congr_thunk ((extRen_comp xivalue zetavalue Eqvalue) s0)
     end
- with extRen_comp { mvalue : nat } { nvalue : nat } (xivalue : fin (mvalue) -> fin (nvalue)) (zetavalue : fin (mvalue) -> fin (nvalue)) (Eqvalue : forall x, xivalue x = zetavalue x) (s : comp (mvalue)) : ren_comp xivalue s = ren_comp zetavalue s :=
-    match s with
+ with extRen_comp { mvalue : nat } { nvalue : nat } (xivalue : (fin) (mvalue) -> (fin) (nvalue)) (zetavalue : (fin) (mvalue) -> (fin) (nvalue)) (Eqvalue : forall x, xivalue x = zetavalue x) (s : comp (mvalue)) : ren_comp xivalue s = ren_comp zetavalue s :=
+    match s return ren_comp xivalue s = ren_comp zetavalue s with
     | cu (_)  => congr_cu 
-    | force (_) s0 => congr_force (extRen_value xivalue zetavalue Eqvalue s0)
-    | lambda (_) s0 => congr_lambda (extRen_comp (upRen_value_value xivalue) (upRen_value_value zetavalue) (upExtRen_value_value (_) (_) Eqvalue) s0)
-    | app (_) s0 s1 => congr_app (extRen_comp xivalue zetavalue Eqvalue s0) (extRen_value xivalue zetavalue Eqvalue s1)
-    | tuple (_) s0 s1 => congr_tuple (extRen_comp xivalue zetavalue Eqvalue s0) (extRen_comp xivalue zetavalue Eqvalue s1)
-    | ret (_) s0 => congr_ret (extRen_value xivalue zetavalue Eqvalue s0)
-    | letin (_) s0 s1 => congr_letin (extRen_comp xivalue zetavalue Eqvalue s0) (extRen_comp (upRen_value_value xivalue) (upRen_value_value zetavalue) (upExtRen_value_value (_) (_) Eqvalue) s1)
-    | proj (_) s0 s1 => congr_proj (eq_refl s0) (extRen_comp xivalue zetavalue Eqvalue s1)
-    | caseZ (_) s0 => congr_caseZ (extRen_value xivalue zetavalue Eqvalue s0)
-    | caseS (_) s0 s1 s2 => congr_caseS (extRen_value xivalue zetavalue Eqvalue s0) (extRen_comp (upRen_value_value xivalue) (upRen_value_value zetavalue) (upExtRen_value_value (_) (_) Eqvalue) s1) (extRen_comp (upRen_value_value xivalue) (upRen_value_value zetavalue) (upExtRen_value_value (_) (_) Eqvalue) s2)
-    | caseP (_) s0 s1 => congr_caseP (extRen_value xivalue zetavalue Eqvalue s0) (extRen_comp (upRen_value_value (upRen_value_value xivalue)) (upRen_value_value (upRen_value_value zetavalue)) (upExtRen_value_value (_) (_) (upExtRen_value_value (_) (_) Eqvalue)) s1)
+    | force (_) s0 => congr_force ((extRen_value xivalue zetavalue Eqvalue) s0)
+    | lambda (_) s0 => congr_lambda ((extRen_comp (upRen_value_value xivalue) (upRen_value_value zetavalue) (upExtRen_value_value (_) (_) Eqvalue)) s0)
+    | app (_) s0 s1 => congr_app ((extRen_comp xivalue zetavalue Eqvalue) s0) ((extRen_value xivalue zetavalue Eqvalue) s1)
+    | tuple (_) s0 s1 => congr_tuple ((extRen_comp xivalue zetavalue Eqvalue) s0) ((extRen_comp xivalue zetavalue Eqvalue) s1)
+    | ret (_) s0 => congr_ret ((extRen_value xivalue zetavalue Eqvalue) s0)
+    | letin (_) s0 s1 => congr_letin ((extRen_comp xivalue zetavalue Eqvalue) s0) ((extRen_comp (upRen_value_value xivalue) (upRen_value_value zetavalue) (upExtRen_value_value (_) (_) Eqvalue)) s1)
+    | proj (_) s0 s1 => congr_proj ((fun x => (eq_refl) x) s0) ((extRen_comp xivalue zetavalue Eqvalue) s1)
+    | caseZ (_) s0 => congr_caseZ ((extRen_value xivalue zetavalue Eqvalue) s0)
+    | caseS (_) s0 s1 s2 => congr_caseS ((extRen_value xivalue zetavalue Eqvalue) s0) ((extRen_comp (upRen_value_value xivalue) (upRen_value_value zetavalue) (upExtRen_value_value (_) (_) Eqvalue)) s1) ((extRen_comp (upRen_value_value xivalue) (upRen_value_value zetavalue) (upExtRen_value_value (_) (_) Eqvalue)) s2)
+    | caseP (_) s0 s1 => congr_caseP ((extRen_value xivalue zetavalue Eqvalue) s0) ((extRen_comp (upRen_value_value (upRen_value_value xivalue)) (upRen_value_value (upRen_value_value zetavalue)) (upExtRen_value_value (_) (_) (upExtRen_value_value (_) (_) Eqvalue))) s1)
     end.
 
-Definition upExt_value_value { m : nat } { nvalue : nat } (sigma : fin (m) -> value (nvalue)) (tau : fin (m) -> value (nvalue)) (Eq : forall x, sigma x = tau x) : forall x, (up_value_value sigma) x = (up_value_value tau) x :=
+Definition upExt_value_value { m : nat } { nvalue : nat } (sigma : (fin) (m) -> value (nvalue)) (tau : (fin) (m) -> value (nvalue)) (Eq : forall x, sigma x = tau x) : forall x, (up_value_value sigma) x = (up_value_value tau) x :=
   fun n => match n with
-  | Some n => ap (ren_value shift) (Eq n)
-  | None => eq_refl
+  | Some fin_n => (ap) (ren_value (shift)) (Eq fin_n)
+  | None  => eq_refl
   end.
 
-Fixpoint ext_value { mvalue : nat } { nvalue : nat } (sigmavalue : fin (mvalue) -> value (nvalue)) (tauvalue : fin (mvalue) -> value (nvalue)) (Eqvalue : forall x, sigmavalue x = tauvalue x) (s : value (mvalue)) : subst_value sigmavalue s = subst_value tauvalue s :=
-    match s with
+Fixpoint ext_value { mvalue : nat } { nvalue : nat } (sigmavalue : (fin) (mvalue) -> value (nvalue)) (tauvalue : (fin) (mvalue) -> value (nvalue)) (Eqvalue : forall x, sigmavalue x = tauvalue x) (s : value (mvalue)) : subst_value sigmavalue s = subst_value tauvalue s :=
+    match s return subst_value sigmavalue s = subst_value tauvalue s with
     | var_value (_) s => Eqvalue s
     | u (_)  => congr_u 
-    | pair (_) s0 s1 => congr_pair (ext_value sigmavalue tauvalue Eqvalue s0) (ext_value sigmavalue tauvalue Eqvalue s1)
-    | inj (_) s0 s1 => congr_inj (eq_refl s0) (ext_value sigmavalue tauvalue Eqvalue s1)
-    | thunk (_) s0 => congr_thunk (ext_comp sigmavalue tauvalue Eqvalue s0)
+    | pair (_) s0 s1 => congr_pair ((ext_value sigmavalue tauvalue Eqvalue) s0) ((ext_value sigmavalue tauvalue Eqvalue) s1)
+    | inj (_) s0 s1 => congr_inj ((fun x => (eq_refl) x) s0) ((ext_value sigmavalue tauvalue Eqvalue) s1)
+    | thunk (_) s0 => congr_thunk ((ext_comp sigmavalue tauvalue Eqvalue) s0)
     end
- with ext_comp { mvalue : nat } { nvalue : nat } (sigmavalue : fin (mvalue) -> value (nvalue)) (tauvalue : fin (mvalue) -> value (nvalue)) (Eqvalue : forall x, sigmavalue x = tauvalue x) (s : comp (mvalue)) : subst_comp sigmavalue s = subst_comp tauvalue s :=
-    match s with
+ with ext_comp { mvalue : nat } { nvalue : nat } (sigmavalue : (fin) (mvalue) -> value (nvalue)) (tauvalue : (fin) (mvalue) -> value (nvalue)) (Eqvalue : forall x, sigmavalue x = tauvalue x) (s : comp (mvalue)) : subst_comp sigmavalue s = subst_comp tauvalue s :=
+    match s return subst_comp sigmavalue s = subst_comp tauvalue s with
     | cu (_)  => congr_cu 
-    | force (_) s0 => congr_force (ext_value sigmavalue tauvalue Eqvalue s0)
-    | lambda (_) s0 => congr_lambda (ext_comp (up_value_value sigmavalue) (up_value_value tauvalue) (upExt_value_value (_) (_) Eqvalue) s0)
-    | app (_) s0 s1 => congr_app (ext_comp sigmavalue tauvalue Eqvalue s0) (ext_value sigmavalue tauvalue Eqvalue s1)
-    | tuple (_) s0 s1 => congr_tuple (ext_comp sigmavalue tauvalue Eqvalue s0) (ext_comp sigmavalue tauvalue Eqvalue s1)
-    | ret (_) s0 => congr_ret (ext_value sigmavalue tauvalue Eqvalue s0)
-    | letin (_) s0 s1 => congr_letin (ext_comp sigmavalue tauvalue Eqvalue s0) (ext_comp (up_value_value sigmavalue) (up_value_value tauvalue) (upExt_value_value (_) (_) Eqvalue) s1)
-    | proj (_) s0 s1 => congr_proj (eq_refl s0) (ext_comp sigmavalue tauvalue Eqvalue s1)
-    | caseZ (_) s0 => congr_caseZ (ext_value sigmavalue tauvalue Eqvalue s0)
-    | caseS (_) s0 s1 s2 => congr_caseS (ext_value sigmavalue tauvalue Eqvalue s0) (ext_comp (up_value_value sigmavalue) (up_value_value tauvalue) (upExt_value_value (_) (_) Eqvalue) s1) (ext_comp (up_value_value sigmavalue) (up_value_value tauvalue) (upExt_value_value (_) (_) Eqvalue) s2)
-    | caseP (_) s0 s1 => congr_caseP (ext_value sigmavalue tauvalue Eqvalue s0) (ext_comp (up_value_value (up_value_value sigmavalue)) (up_value_value (up_value_value tauvalue)) (upExt_value_value (_) (_) (upExt_value_value (_) (_) Eqvalue)) s1)
+    | force (_) s0 => congr_force ((ext_value sigmavalue tauvalue Eqvalue) s0)
+    | lambda (_) s0 => congr_lambda ((ext_comp (up_value_value sigmavalue) (up_value_value tauvalue) (upExt_value_value (_) (_) Eqvalue)) s0)
+    | app (_) s0 s1 => congr_app ((ext_comp sigmavalue tauvalue Eqvalue) s0) ((ext_value sigmavalue tauvalue Eqvalue) s1)
+    | tuple (_) s0 s1 => congr_tuple ((ext_comp sigmavalue tauvalue Eqvalue) s0) ((ext_comp sigmavalue tauvalue Eqvalue) s1)
+    | ret (_) s0 => congr_ret ((ext_value sigmavalue tauvalue Eqvalue) s0)
+    | letin (_) s0 s1 => congr_letin ((ext_comp sigmavalue tauvalue Eqvalue) s0) ((ext_comp (up_value_value sigmavalue) (up_value_value tauvalue) (upExt_value_value (_) (_) Eqvalue)) s1)
+    | proj (_) s0 s1 => congr_proj ((fun x => (eq_refl) x) s0) ((ext_comp sigmavalue tauvalue Eqvalue) s1)
+    | caseZ (_) s0 => congr_caseZ ((ext_value sigmavalue tauvalue Eqvalue) s0)
+    | caseS (_) s0 s1 s2 => congr_caseS ((ext_value sigmavalue tauvalue Eqvalue) s0) ((ext_comp (up_value_value sigmavalue) (up_value_value tauvalue) (upExt_value_value (_) (_) Eqvalue)) s1) ((ext_comp (up_value_value sigmavalue) (up_value_value tauvalue) (upExt_value_value (_) (_) Eqvalue)) s2)
+    | caseP (_) s0 s1 => congr_caseP ((ext_value sigmavalue tauvalue Eqvalue) s0) ((ext_comp (up_value_value (up_value_value sigmavalue)) (up_value_value (up_value_value tauvalue)) (upExt_value_value (_) (_) (upExt_value_value (_) (_) Eqvalue))) s1)
     end.
 
-Fixpoint compRenRen_value { kvalue : nat } { lvalue : nat } { mvalue : nat } (xivalue : fin (mvalue) -> fin (kvalue)) (zetavalue : fin (kvalue) -> fin (lvalue)) (rhovalue : fin (mvalue) -> fin (lvalue)) (Eqvalue : forall x, (funcomp zetavalue xivalue) x = rhovalue x) (s : value (mvalue)) : ren_value zetavalue (ren_value xivalue s) = ren_value rhovalue s :=
-    match s with
-    | var_value (_) s => ap (var_value (lvalue)) (Eqvalue s)
+Definition up_ren_ren_value_value { k : nat } { l : nat } { m : nat } (xi : (fin) (k) -> (fin) (l)) (tau : (fin) (l) -> (fin) (m)) (theta : (fin) (k) -> (fin) (m)) (Eq : forall x, ((funcomp) tau xi) x = theta x) : forall x, ((funcomp) (upRen_value_value tau) (upRen_value_value xi)) x = (upRen_value_value theta) x :=
+  up_ren_ren xi tau theta Eq.
+
+Fixpoint compRenRen_value { kvalue : nat } { lvalue : nat } { mvalue : nat } (xivalue : (fin) (mvalue) -> (fin) (kvalue)) (zetavalue : (fin) (kvalue) -> (fin) (lvalue)) (rhovalue : (fin) (mvalue) -> (fin) (lvalue)) (Eqvalue : forall x, ((funcomp) zetavalue xivalue) x = rhovalue x) (s : value (mvalue)) : ren_value zetavalue (ren_value xivalue s) = ren_value rhovalue s :=
+    match s return ren_value zetavalue (ren_value xivalue s) = ren_value rhovalue s with
+    | var_value (_) s => (ap) (var_value (lvalue)) (Eqvalue s)
     | u (_)  => congr_u 
-    | pair (_) s0 s1 => congr_pair (compRenRen_value xivalue zetavalue rhovalue Eqvalue s0) (compRenRen_value xivalue zetavalue rhovalue Eqvalue s1)
-    | inj (_) s0 s1 => congr_inj (eq_refl s0) (compRenRen_value xivalue zetavalue rhovalue Eqvalue s1)
-    | thunk (_) s0 => congr_thunk (compRenRen_comp xivalue zetavalue rhovalue Eqvalue s0)
+    | pair (_) s0 s1 => congr_pair ((compRenRen_value xivalue zetavalue rhovalue Eqvalue) s0) ((compRenRen_value xivalue zetavalue rhovalue Eqvalue) s1)
+    | inj (_) s0 s1 => congr_inj ((fun x => (eq_refl) x) s0) ((compRenRen_value xivalue zetavalue rhovalue Eqvalue) s1)
+    | thunk (_) s0 => congr_thunk ((compRenRen_comp xivalue zetavalue rhovalue Eqvalue) s0)
     end
- with compRenRen_comp { kvalue : nat } { lvalue : nat } { mvalue : nat } (xivalue : fin (mvalue) -> fin (kvalue)) (zetavalue : fin (kvalue) -> fin (lvalue)) (rhovalue : fin (mvalue) -> fin (lvalue)) (Eqvalue : forall x, (funcomp zetavalue xivalue) x = rhovalue x) (s : comp (mvalue)) : ren_comp zetavalue (ren_comp xivalue s) = ren_comp rhovalue s :=
-    match s with
+ with compRenRen_comp { kvalue : nat } { lvalue : nat } { mvalue : nat } (xivalue : (fin) (mvalue) -> (fin) (kvalue)) (zetavalue : (fin) (kvalue) -> (fin) (lvalue)) (rhovalue : (fin) (mvalue) -> (fin) (lvalue)) (Eqvalue : forall x, ((funcomp) zetavalue xivalue) x = rhovalue x) (s : comp (mvalue)) : ren_comp zetavalue (ren_comp xivalue s) = ren_comp rhovalue s :=
+    match s return ren_comp zetavalue (ren_comp xivalue s) = ren_comp rhovalue s with
     | cu (_)  => congr_cu 
-    | force (_) s0 => congr_force (compRenRen_value xivalue zetavalue rhovalue Eqvalue s0)
-    | lambda (_) s0 => congr_lambda (compRenRen_comp (upRen_value_value xivalue) (upRen_value_value zetavalue) (upRen_value_value rhovalue) (up_ren_ren (_) (_) (_) Eqvalue) s0)
-    | app (_) s0 s1 => congr_app (compRenRen_comp xivalue zetavalue rhovalue Eqvalue s0) (compRenRen_value xivalue zetavalue rhovalue Eqvalue s1)
-    | tuple (_) s0 s1 => congr_tuple (compRenRen_comp xivalue zetavalue rhovalue Eqvalue s0) (compRenRen_comp xivalue zetavalue rhovalue Eqvalue s1)
-    | ret (_) s0 => congr_ret (compRenRen_value xivalue zetavalue rhovalue Eqvalue s0)
-    | letin (_) s0 s1 => congr_letin (compRenRen_comp xivalue zetavalue rhovalue Eqvalue s0) (compRenRen_comp (upRen_value_value xivalue) (upRen_value_value zetavalue) (upRen_value_value rhovalue) (up_ren_ren (_) (_) (_) Eqvalue) s1)
-    | proj (_) s0 s1 => congr_proj (eq_refl s0) (compRenRen_comp xivalue zetavalue rhovalue Eqvalue s1)
-    | caseZ (_) s0 => congr_caseZ (compRenRen_value xivalue zetavalue rhovalue Eqvalue s0)
-    | caseS (_) s0 s1 s2 => congr_caseS (compRenRen_value xivalue zetavalue rhovalue Eqvalue s0) (compRenRen_comp (upRen_value_value xivalue) (upRen_value_value zetavalue) (upRen_value_value rhovalue) (up_ren_ren (_) (_) (_) Eqvalue) s1) (compRenRen_comp (upRen_value_value xivalue) (upRen_value_value zetavalue) (upRen_value_value rhovalue) (up_ren_ren (_) (_) (_) Eqvalue) s2)
-    | caseP (_) s0 s1 => congr_caseP (compRenRen_value xivalue zetavalue rhovalue Eqvalue s0) (compRenRen_comp (upRen_value_value (upRen_value_value xivalue)) (upRen_value_value (upRen_value_value zetavalue)) (upRen_value_value (upRen_value_value rhovalue)) (up_ren_ren (_) (_) (_) (up_ren_ren (_) (_) (_) Eqvalue)) s1)
+    | force (_) s0 => congr_force ((compRenRen_value xivalue zetavalue rhovalue Eqvalue) s0)
+    | lambda (_) s0 => congr_lambda ((compRenRen_comp (upRen_value_value xivalue) (upRen_value_value zetavalue) (upRen_value_value rhovalue) (up_ren_ren (_) (_) (_) Eqvalue)) s0)
+    | app (_) s0 s1 => congr_app ((compRenRen_comp xivalue zetavalue rhovalue Eqvalue) s0) ((compRenRen_value xivalue zetavalue rhovalue Eqvalue) s1)
+    | tuple (_) s0 s1 => congr_tuple ((compRenRen_comp xivalue zetavalue rhovalue Eqvalue) s0) ((compRenRen_comp xivalue zetavalue rhovalue Eqvalue) s1)
+    | ret (_) s0 => congr_ret ((compRenRen_value xivalue zetavalue rhovalue Eqvalue) s0)
+    | letin (_) s0 s1 => congr_letin ((compRenRen_comp xivalue zetavalue rhovalue Eqvalue) s0) ((compRenRen_comp (upRen_value_value xivalue) (upRen_value_value zetavalue) (upRen_value_value rhovalue) (up_ren_ren (_) (_) (_) Eqvalue)) s1)
+    | proj (_) s0 s1 => congr_proj ((fun x => (eq_refl) x) s0) ((compRenRen_comp xivalue zetavalue rhovalue Eqvalue) s1)
+    | caseZ (_) s0 => congr_caseZ ((compRenRen_value xivalue zetavalue rhovalue Eqvalue) s0)
+    | caseS (_) s0 s1 s2 => congr_caseS ((compRenRen_value xivalue zetavalue rhovalue Eqvalue) s0) ((compRenRen_comp (upRen_value_value xivalue) (upRen_value_value zetavalue) (upRen_value_value rhovalue) (up_ren_ren (_) (_) (_) Eqvalue)) s1) ((compRenRen_comp (upRen_value_value xivalue) (upRen_value_value zetavalue) (upRen_value_value rhovalue) (up_ren_ren (_) (_) (_) Eqvalue)) s2)
+    | caseP (_) s0 s1 => congr_caseP ((compRenRen_value xivalue zetavalue rhovalue Eqvalue) s0) ((compRenRen_comp (upRen_value_value (upRen_value_value xivalue)) (upRen_value_value (upRen_value_value zetavalue)) (upRen_value_value (upRen_value_value rhovalue)) (up_ren_ren (_) (_) (_) (up_ren_ren (_) (_) (_) Eqvalue))) s1)
     end.
 
-Definition up_ren_subst_value_value { k : nat } { l : nat } { mvalue : nat } (xi : fin (k) -> fin (l)) (tau : fin (l) -> value (mvalue)) (theta : fin (k) -> value (mvalue)) (Eq : forall x, (funcomp tau xi) x = theta x) : forall x, (funcomp (up_value_value tau) (upRen_value_value xi)) x = (up_value_value theta) x :=
+Definition up_ren_subst_value_value { k : nat } { l : nat } { mvalue : nat } (xi : (fin) (k) -> (fin) (l)) (tau : (fin) (l) -> value (mvalue)) (theta : (fin) (k) -> value (mvalue)) (Eq : forall x, ((funcomp) tau xi) x = theta x) : forall x, ((funcomp) (up_value_value tau) (upRen_value_value xi)) x = (up_value_value theta) x :=
   fun n => match n with
-  | Some n => ap (ren_value shift) (Eq n)
-  | None => eq_refl
+  | Some fin_n => (ap) (ren_value (shift)) (Eq fin_n)
+  | None  => eq_refl
   end.
 
-Fixpoint compRenSubst_value { kvalue : nat } { lvalue : nat } { mvalue : nat } (xivalue : fin (mvalue) -> fin (kvalue)) (tauvalue : fin (kvalue) -> value (lvalue)) (thetavalue : fin (mvalue) -> value (lvalue)) (Eqvalue : forall x, (funcomp tauvalue xivalue) x = thetavalue x) (s : value (mvalue)) : subst_value tauvalue (ren_value xivalue s) = subst_value thetavalue s :=
-    match s with
+Fixpoint compRenSubst_value { kvalue : nat } { lvalue : nat } { mvalue : nat } (xivalue : (fin) (mvalue) -> (fin) (kvalue)) (tauvalue : (fin) (kvalue) -> value (lvalue)) (thetavalue : (fin) (mvalue) -> value (lvalue)) (Eqvalue : forall x, ((funcomp) tauvalue xivalue) x = thetavalue x) (s : value (mvalue)) : subst_value tauvalue (ren_value xivalue s) = subst_value thetavalue s :=
+    match s return subst_value tauvalue (ren_value xivalue s) = subst_value thetavalue s with
     | var_value (_) s => Eqvalue s
     | u (_)  => congr_u 
-    | pair (_) s0 s1 => congr_pair (compRenSubst_value xivalue tauvalue thetavalue Eqvalue s0) (compRenSubst_value xivalue tauvalue thetavalue Eqvalue s1)
-    | inj (_) s0 s1 => congr_inj (eq_refl s0) (compRenSubst_value xivalue tauvalue thetavalue Eqvalue s1)
-    | thunk (_) s0 => congr_thunk (compRenSubst_comp xivalue tauvalue thetavalue Eqvalue s0)
+    | pair (_) s0 s1 => congr_pair ((compRenSubst_value xivalue tauvalue thetavalue Eqvalue) s0) ((compRenSubst_value xivalue tauvalue thetavalue Eqvalue) s1)
+    | inj (_) s0 s1 => congr_inj ((fun x => (eq_refl) x) s0) ((compRenSubst_value xivalue tauvalue thetavalue Eqvalue) s1)
+    | thunk (_) s0 => congr_thunk ((compRenSubst_comp xivalue tauvalue thetavalue Eqvalue) s0)
     end
- with compRenSubst_comp { kvalue : nat } { lvalue : nat } { mvalue : nat } (xivalue : fin (mvalue) -> fin (kvalue)) (tauvalue : fin (kvalue) -> value (lvalue)) (thetavalue : fin (mvalue) -> value (lvalue)) (Eqvalue : forall x, (funcomp tauvalue xivalue) x = thetavalue x) (s : comp (mvalue)) : subst_comp tauvalue (ren_comp xivalue s) = subst_comp thetavalue s :=
-    match s with
+ with compRenSubst_comp { kvalue : nat } { lvalue : nat } { mvalue : nat } (xivalue : (fin) (mvalue) -> (fin) (kvalue)) (tauvalue : (fin) (kvalue) -> value (lvalue)) (thetavalue : (fin) (mvalue) -> value (lvalue)) (Eqvalue : forall x, ((funcomp) tauvalue xivalue) x = thetavalue x) (s : comp (mvalue)) : subst_comp tauvalue (ren_comp xivalue s) = subst_comp thetavalue s :=
+    match s return subst_comp tauvalue (ren_comp xivalue s) = subst_comp thetavalue s with
     | cu (_)  => congr_cu 
-    | force (_) s0 => congr_force (compRenSubst_value xivalue tauvalue thetavalue Eqvalue s0)
-    | lambda (_) s0 => congr_lambda (compRenSubst_comp (upRen_value_value xivalue) (up_value_value tauvalue) (up_value_value thetavalue) (up_ren_subst_value_value (_) (_) (_) Eqvalue) s0)
-    | app (_) s0 s1 => congr_app (compRenSubst_comp xivalue tauvalue thetavalue Eqvalue s0) (compRenSubst_value xivalue tauvalue thetavalue Eqvalue s1)
-    | tuple (_) s0 s1 => congr_tuple (compRenSubst_comp xivalue tauvalue thetavalue Eqvalue s0) (compRenSubst_comp xivalue tauvalue thetavalue Eqvalue s1)
-    | ret (_) s0 => congr_ret (compRenSubst_value xivalue tauvalue thetavalue Eqvalue s0)
-    | letin (_) s0 s1 => congr_letin (compRenSubst_comp xivalue tauvalue thetavalue Eqvalue s0) (compRenSubst_comp (upRen_value_value xivalue) (up_value_value tauvalue) (up_value_value thetavalue) (up_ren_subst_value_value (_) (_) (_) Eqvalue) s1)
-    | proj (_) s0 s1 => congr_proj (eq_refl s0) (compRenSubst_comp xivalue tauvalue thetavalue Eqvalue s1)
-    | caseZ (_) s0 => congr_caseZ (compRenSubst_value xivalue tauvalue thetavalue Eqvalue s0)
-    | caseS (_) s0 s1 s2 => congr_caseS (compRenSubst_value xivalue tauvalue thetavalue Eqvalue s0) (compRenSubst_comp (upRen_value_value xivalue) (up_value_value tauvalue) (up_value_value thetavalue) (up_ren_subst_value_value (_) (_) (_) Eqvalue) s1) (compRenSubst_comp (upRen_value_value xivalue) (up_value_value tauvalue) (up_value_value thetavalue) (up_ren_subst_value_value (_) (_) (_) Eqvalue) s2)
-    | caseP (_) s0 s1 => congr_caseP (compRenSubst_value xivalue tauvalue thetavalue Eqvalue s0) (compRenSubst_comp (upRen_value_value (upRen_value_value xivalue)) (up_value_value (up_value_value tauvalue)) (up_value_value (up_value_value thetavalue)) (up_ren_subst_value_value (_) (_) (_) (up_ren_subst_value_value (_) (_) (_) Eqvalue)) s1)
+    | force (_) s0 => congr_force ((compRenSubst_value xivalue tauvalue thetavalue Eqvalue) s0)
+    | lambda (_) s0 => congr_lambda ((compRenSubst_comp (upRen_value_value xivalue) (up_value_value tauvalue) (up_value_value thetavalue) (up_ren_subst_value_value (_) (_) (_) Eqvalue)) s0)
+    | app (_) s0 s1 => congr_app ((compRenSubst_comp xivalue tauvalue thetavalue Eqvalue) s0) ((compRenSubst_value xivalue tauvalue thetavalue Eqvalue) s1)
+    | tuple (_) s0 s1 => congr_tuple ((compRenSubst_comp xivalue tauvalue thetavalue Eqvalue) s0) ((compRenSubst_comp xivalue tauvalue thetavalue Eqvalue) s1)
+    | ret (_) s0 => congr_ret ((compRenSubst_value xivalue tauvalue thetavalue Eqvalue) s0)
+    | letin (_) s0 s1 => congr_letin ((compRenSubst_comp xivalue tauvalue thetavalue Eqvalue) s0) ((compRenSubst_comp (upRen_value_value xivalue) (up_value_value tauvalue) (up_value_value thetavalue) (up_ren_subst_value_value (_) (_) (_) Eqvalue)) s1)
+    | proj (_) s0 s1 => congr_proj ((fun x => (eq_refl) x) s0) ((compRenSubst_comp xivalue tauvalue thetavalue Eqvalue) s1)
+    | caseZ (_) s0 => congr_caseZ ((compRenSubst_value xivalue tauvalue thetavalue Eqvalue) s0)
+    | caseS (_) s0 s1 s2 => congr_caseS ((compRenSubst_value xivalue tauvalue thetavalue Eqvalue) s0) ((compRenSubst_comp (upRen_value_value xivalue) (up_value_value tauvalue) (up_value_value thetavalue) (up_ren_subst_value_value (_) (_) (_) Eqvalue)) s1) ((compRenSubst_comp (upRen_value_value xivalue) (up_value_value tauvalue) (up_value_value thetavalue) (up_ren_subst_value_value (_) (_) (_) Eqvalue)) s2)
+    | caseP (_) s0 s1 => congr_caseP ((compRenSubst_value xivalue tauvalue thetavalue Eqvalue) s0) ((compRenSubst_comp (upRen_value_value (upRen_value_value xivalue)) (up_value_value (up_value_value tauvalue)) (up_value_value (up_value_value thetavalue)) (up_ren_subst_value_value (_) (_) (_) (up_ren_subst_value_value (_) (_) (_) Eqvalue))) s1)
     end.
 
-Definition up_subst_ren_value_value { k : nat } { lvalue : nat } { mvalue : nat } (sigma : fin (k) -> value (lvalue)) (zetavalue : fin (lvalue) -> fin (mvalue)) (theta : fin (k) -> value (mvalue)) (Eq : forall x, (funcomp (ren_value zetavalue) sigma) x = theta x) : forall x, (funcomp (ren_value (upRen_value_value zetavalue)) (up_value_value sigma)) x = (up_value_value theta) x :=
+Definition up_subst_ren_value_value { k : nat } { lvalue : nat } { mvalue : nat } (sigma : (fin) (k) -> value (lvalue)) (zetavalue : (fin) (lvalue) -> (fin) (mvalue)) (theta : (fin) (k) -> value (mvalue)) (Eq : forall x, ((funcomp) (ren_value zetavalue) sigma) x = theta x) : forall x, ((funcomp) (ren_value (upRen_value_value zetavalue)) (up_value_value sigma)) x = (up_value_value theta) x :=
   fun n => match n with
-  | Some n => eq_trans (compRenRen_value shift (upRen_value_value zetavalue) (funcomp shift zetavalue) (fun x => eq_refl) (sigma n)) (eq_trans (eq_sym (compRenRen_value zetavalue shift (funcomp shift zetavalue) (fun x => eq_refl) (sigma n))) (ap (ren_value shift) (Eq n)))
-  | None => eq_refl
+  | Some fin_n => (eq_trans) (compRenRen_value (shift) (upRen_value_value zetavalue) ((funcomp) (shift) zetavalue) (fun x => eq_refl) (sigma fin_n)) ((eq_trans) ((eq_sym) (compRenRen_value zetavalue (shift) ((funcomp) (shift) zetavalue) (fun x => eq_refl) (sigma fin_n))) ((ap) (ren_value (shift)) (Eq fin_n)))
+  | None  => eq_refl
   end.
 
-Fixpoint compSubstRen__value { kvalue : nat } { lvalue : nat } { mvalue : nat } (sigmavalue : fin (mvalue) -> value (kvalue)) (zetavalue : fin (kvalue) -> fin (lvalue)) (thetavalue : fin (mvalue) -> value (lvalue)) (Eqvalue : forall x, (funcomp (ren_value zetavalue) sigmavalue) x = thetavalue x) (s : value (mvalue)) : ren_value zetavalue (subst_value sigmavalue s) = subst_value thetavalue s :=
-    match s with
+Fixpoint compSubstRen_value { kvalue : nat } { lvalue : nat } { mvalue : nat } (sigmavalue : (fin) (mvalue) -> value (kvalue)) (zetavalue : (fin) (kvalue) -> (fin) (lvalue)) (thetavalue : (fin) (mvalue) -> value (lvalue)) (Eqvalue : forall x, ((funcomp) (ren_value zetavalue) sigmavalue) x = thetavalue x) (s : value (mvalue)) : ren_value zetavalue (subst_value sigmavalue s) = subst_value thetavalue s :=
+    match s return ren_value zetavalue (subst_value sigmavalue s) = subst_value thetavalue s with
     | var_value (_) s => Eqvalue s
     | u (_)  => congr_u 
-    | pair (_) s0 s1 => congr_pair (compSubstRen__value sigmavalue zetavalue thetavalue Eqvalue s0) (compSubstRen__value sigmavalue zetavalue thetavalue Eqvalue s1)
-    | inj (_) s0 s1 => congr_inj (eq_refl s0) (compSubstRen__value sigmavalue zetavalue thetavalue Eqvalue s1)
-    | thunk (_) s0 => congr_thunk (compSubstRen__comp sigmavalue zetavalue thetavalue Eqvalue s0)
+    | pair (_) s0 s1 => congr_pair ((compSubstRen_value sigmavalue zetavalue thetavalue Eqvalue) s0) ((compSubstRen_value sigmavalue zetavalue thetavalue Eqvalue) s1)
+    | inj (_) s0 s1 => congr_inj ((fun x => (eq_refl) x) s0) ((compSubstRen_value sigmavalue zetavalue thetavalue Eqvalue) s1)
+    | thunk (_) s0 => congr_thunk ((compSubstRen_comp sigmavalue zetavalue thetavalue Eqvalue) s0)
     end
- with compSubstRen__comp { kvalue : nat } { lvalue : nat } { mvalue : nat } (sigmavalue : fin (mvalue) -> value (kvalue)) (zetavalue : fin (kvalue) -> fin (lvalue)) (thetavalue : fin (mvalue) -> value (lvalue)) (Eqvalue : forall x, (funcomp (ren_value zetavalue) sigmavalue) x = thetavalue x) (s : comp (mvalue)) : ren_comp zetavalue (subst_comp sigmavalue s) = subst_comp thetavalue s :=
-    match s with
+ with compSubstRen_comp { kvalue : nat } { lvalue : nat } { mvalue : nat } (sigmavalue : (fin) (mvalue) -> value (kvalue)) (zetavalue : (fin) (kvalue) -> (fin) (lvalue)) (thetavalue : (fin) (mvalue) -> value (lvalue)) (Eqvalue : forall x, ((funcomp) (ren_value zetavalue) sigmavalue) x = thetavalue x) (s : comp (mvalue)) : ren_comp zetavalue (subst_comp sigmavalue s) = subst_comp thetavalue s :=
+    match s return ren_comp zetavalue (subst_comp sigmavalue s) = subst_comp thetavalue s with
     | cu (_)  => congr_cu 
-    | force (_) s0 => congr_force (compSubstRen__value sigmavalue zetavalue thetavalue Eqvalue s0)
-    | lambda (_) s0 => congr_lambda (compSubstRen__comp (up_value_value sigmavalue) (upRen_value_value zetavalue) (up_value_value thetavalue) (up_subst_ren_value_value (_) (_) (_) Eqvalue) s0)
-    | app (_) s0 s1 => congr_app (compSubstRen__comp sigmavalue zetavalue thetavalue Eqvalue s0) (compSubstRen__value sigmavalue zetavalue thetavalue Eqvalue s1)
-    | tuple (_) s0 s1 => congr_tuple (compSubstRen__comp sigmavalue zetavalue thetavalue Eqvalue s0) (compSubstRen__comp sigmavalue zetavalue thetavalue Eqvalue s1)
-    | ret (_) s0 => congr_ret (compSubstRen__value sigmavalue zetavalue thetavalue Eqvalue s0)
-    | letin (_) s0 s1 => congr_letin (compSubstRen__comp sigmavalue zetavalue thetavalue Eqvalue s0) (compSubstRen__comp (up_value_value sigmavalue) (upRen_value_value zetavalue) (up_value_value thetavalue) (up_subst_ren_value_value (_) (_) (_) Eqvalue) s1)
-    | proj (_) s0 s1 => congr_proj (eq_refl s0) (compSubstRen__comp sigmavalue zetavalue thetavalue Eqvalue s1)
-    | caseZ (_) s0 => congr_caseZ (compSubstRen__value sigmavalue zetavalue thetavalue Eqvalue s0)
-    | caseS (_) s0 s1 s2 => congr_caseS (compSubstRen__value sigmavalue zetavalue thetavalue Eqvalue s0) (compSubstRen__comp (up_value_value sigmavalue) (upRen_value_value zetavalue) (up_value_value thetavalue) (up_subst_ren_value_value (_) (_) (_) Eqvalue) s1) (compSubstRen__comp (up_value_value sigmavalue) (upRen_value_value zetavalue) (up_value_value thetavalue) (up_subst_ren_value_value (_) (_) (_) Eqvalue) s2)
-    | caseP (_) s0 s1 => congr_caseP (compSubstRen__value sigmavalue zetavalue thetavalue Eqvalue s0) (compSubstRen__comp (up_value_value (up_value_value sigmavalue)) (upRen_value_value (upRen_value_value zetavalue)) (up_value_value (up_value_value thetavalue)) (up_subst_ren_value_value (_) (_) (_) (up_subst_ren_value_value (_) (_) (_) Eqvalue)) s1)
+    | force (_) s0 => congr_force ((compSubstRen_value sigmavalue zetavalue thetavalue Eqvalue) s0)
+    | lambda (_) s0 => congr_lambda ((compSubstRen_comp (up_value_value sigmavalue) (upRen_value_value zetavalue) (up_value_value thetavalue) (up_subst_ren_value_value (_) (_) (_) Eqvalue)) s0)
+    | app (_) s0 s1 => congr_app ((compSubstRen_comp sigmavalue zetavalue thetavalue Eqvalue) s0) ((compSubstRen_value sigmavalue zetavalue thetavalue Eqvalue) s1)
+    | tuple (_) s0 s1 => congr_tuple ((compSubstRen_comp sigmavalue zetavalue thetavalue Eqvalue) s0) ((compSubstRen_comp sigmavalue zetavalue thetavalue Eqvalue) s1)
+    | ret (_) s0 => congr_ret ((compSubstRen_value sigmavalue zetavalue thetavalue Eqvalue) s0)
+    | letin (_) s0 s1 => congr_letin ((compSubstRen_comp sigmavalue zetavalue thetavalue Eqvalue) s0) ((compSubstRen_comp (up_value_value sigmavalue) (upRen_value_value zetavalue) (up_value_value thetavalue) (up_subst_ren_value_value (_) (_) (_) Eqvalue)) s1)
+    | proj (_) s0 s1 => congr_proj ((fun x => (eq_refl) x) s0) ((compSubstRen_comp sigmavalue zetavalue thetavalue Eqvalue) s1)
+    | caseZ (_) s0 => congr_caseZ ((compSubstRen_value sigmavalue zetavalue thetavalue Eqvalue) s0)
+    | caseS (_) s0 s1 s2 => congr_caseS ((compSubstRen_value sigmavalue zetavalue thetavalue Eqvalue) s0) ((compSubstRen_comp (up_value_value sigmavalue) (upRen_value_value zetavalue) (up_value_value thetavalue) (up_subst_ren_value_value (_) (_) (_) Eqvalue)) s1) ((compSubstRen_comp (up_value_value sigmavalue) (upRen_value_value zetavalue) (up_value_value thetavalue) (up_subst_ren_value_value (_) (_) (_) Eqvalue)) s2)
+    | caseP (_) s0 s1 => congr_caseP ((compSubstRen_value sigmavalue zetavalue thetavalue Eqvalue) s0) ((compSubstRen_comp (up_value_value (up_value_value sigmavalue)) (upRen_value_value (upRen_value_value zetavalue)) (up_value_value (up_value_value thetavalue)) (up_subst_ren_value_value (_) (_) (_) (up_subst_ren_value_value (_) (_) (_) Eqvalue))) s1)
     end.
 
-Definition up_subst_subst_value_value { k : nat } { lvalue : nat } { mvalue : nat } (sigma : fin (k) -> value (lvalue)) (tauvalue : fin (lvalue) -> value (mvalue)) (theta : fin (k) -> value (mvalue)) (Eq : forall x, (funcomp (subst_value tauvalue) sigma) x = theta x) : forall x, (funcomp (subst_value (up_value_value tauvalue)) (up_value_value sigma)) x = (up_value_value theta) x :=
+Definition up_subst_subst_value_value { k : nat } { lvalue : nat } { mvalue : nat } (sigma : (fin) (k) -> value (lvalue)) (tauvalue : (fin) (lvalue) -> value (mvalue)) (theta : (fin) (k) -> value (mvalue)) (Eq : forall x, ((funcomp) (subst_value tauvalue) sigma) x = theta x) : forall x, ((funcomp) (subst_value (up_value_value tauvalue)) (up_value_value sigma)) x = (up_value_value theta) x :=
   fun n => match n with
-  | Some n => eq_trans (compRenSubst_value shift (up_value_value tauvalue) (funcomp (up_value_value tauvalue) shift) (fun x => eq_refl) (sigma n)) (eq_trans (eq_sym (compSubstRen__value tauvalue shift (funcomp (ren_value shift) tauvalue) (fun x => eq_refl) (sigma n))) (ap (ren_value shift) (Eq n)))
-  | None => eq_refl
+  | Some fin_n => (eq_trans) (compRenSubst_value (shift) (up_value_value tauvalue) ((funcomp) (up_value_value tauvalue) (shift)) (fun x => eq_refl) (sigma fin_n)) ((eq_trans) ((eq_sym) (compSubstRen_value tauvalue (shift) ((funcomp) (ren_value (shift)) tauvalue) (fun x => eq_refl) (sigma fin_n))) ((ap) (ren_value (shift)) (Eq fin_n)))
+  | None  => eq_refl
   end.
 
-Fixpoint compSubstSubst_value { kvalue : nat } { lvalue : nat } { mvalue : nat } (sigmavalue : fin (mvalue) -> value (kvalue)) (tauvalue : fin (kvalue) -> value (lvalue)) (thetavalue : fin (mvalue) -> value (lvalue)) (Eqvalue : forall x, (funcomp (subst_value tauvalue) sigmavalue) x = thetavalue x) (s : value (mvalue)) : subst_value tauvalue (subst_value sigmavalue s) = subst_value thetavalue s :=
-    match s with
+Fixpoint compSubstSubst_value { kvalue : nat } { lvalue : nat } { mvalue : nat } (sigmavalue : (fin) (mvalue) -> value (kvalue)) (tauvalue : (fin) (kvalue) -> value (lvalue)) (thetavalue : (fin) (mvalue) -> value (lvalue)) (Eqvalue : forall x, ((funcomp) (subst_value tauvalue) sigmavalue) x = thetavalue x) (s : value (mvalue)) : subst_value tauvalue (subst_value sigmavalue s) = subst_value thetavalue s :=
+    match s return subst_value tauvalue (subst_value sigmavalue s) = subst_value thetavalue s with
     | var_value (_) s => Eqvalue s
     | u (_)  => congr_u 
-    | pair (_) s0 s1 => congr_pair (compSubstSubst_value sigmavalue tauvalue thetavalue Eqvalue s0) (compSubstSubst_value sigmavalue tauvalue thetavalue Eqvalue s1)
-    | inj (_) s0 s1 => congr_inj (eq_refl s0) (compSubstSubst_value sigmavalue tauvalue thetavalue Eqvalue s1)
-    | thunk (_) s0 => congr_thunk (compSubstSubst_comp sigmavalue tauvalue thetavalue Eqvalue s0)
+    | pair (_) s0 s1 => congr_pair ((compSubstSubst_value sigmavalue tauvalue thetavalue Eqvalue) s0) ((compSubstSubst_value sigmavalue tauvalue thetavalue Eqvalue) s1)
+    | inj (_) s0 s1 => congr_inj ((fun x => (eq_refl) x) s0) ((compSubstSubst_value sigmavalue tauvalue thetavalue Eqvalue) s1)
+    | thunk (_) s0 => congr_thunk ((compSubstSubst_comp sigmavalue tauvalue thetavalue Eqvalue) s0)
     end
- with compSubstSubst_comp { kvalue : nat } { lvalue : nat } { mvalue : nat } (sigmavalue : fin (mvalue) -> value (kvalue)) (tauvalue : fin (kvalue) -> value (lvalue)) (thetavalue : fin (mvalue) -> value (lvalue)) (Eqvalue : forall x, (funcomp (subst_value tauvalue) sigmavalue) x = thetavalue x) (s : comp (mvalue)) : subst_comp tauvalue (subst_comp sigmavalue s) = subst_comp thetavalue s :=
-    match s with
+ with compSubstSubst_comp { kvalue : nat } { lvalue : nat } { mvalue : nat } (sigmavalue : (fin) (mvalue) -> value (kvalue)) (tauvalue : (fin) (kvalue) -> value (lvalue)) (thetavalue : (fin) (mvalue) -> value (lvalue)) (Eqvalue : forall x, ((funcomp) (subst_value tauvalue) sigmavalue) x = thetavalue x) (s : comp (mvalue)) : subst_comp tauvalue (subst_comp sigmavalue s) = subst_comp thetavalue s :=
+    match s return subst_comp tauvalue (subst_comp sigmavalue s) = subst_comp thetavalue s with
     | cu (_)  => congr_cu 
-    | force (_) s0 => congr_force (compSubstSubst_value sigmavalue tauvalue thetavalue Eqvalue s0)
-    | lambda (_) s0 => congr_lambda (compSubstSubst_comp (up_value_value sigmavalue) (up_value_value tauvalue) (up_value_value thetavalue) (up_subst_subst_value_value (_) (_) (_) Eqvalue) s0)
-    | app (_) s0 s1 => congr_app (compSubstSubst_comp sigmavalue tauvalue thetavalue Eqvalue s0) (compSubstSubst_value sigmavalue tauvalue thetavalue Eqvalue s1)
-    | tuple (_) s0 s1 => congr_tuple (compSubstSubst_comp sigmavalue tauvalue thetavalue Eqvalue s0) (compSubstSubst_comp sigmavalue tauvalue thetavalue Eqvalue s1)
-    | ret (_) s0 => congr_ret (compSubstSubst_value sigmavalue tauvalue thetavalue Eqvalue s0)
-    | letin (_) s0 s1 => congr_letin (compSubstSubst_comp sigmavalue tauvalue thetavalue Eqvalue s0) (compSubstSubst_comp (up_value_value sigmavalue) (up_value_value tauvalue) (up_value_value thetavalue) (up_subst_subst_value_value (_) (_) (_) Eqvalue) s1)
-    | proj (_) s0 s1 => congr_proj (eq_refl s0) (compSubstSubst_comp sigmavalue tauvalue thetavalue Eqvalue s1)
-    | caseZ (_) s0 => congr_caseZ (compSubstSubst_value sigmavalue tauvalue thetavalue Eqvalue s0)
-    | caseS (_) s0 s1 s2 => congr_caseS (compSubstSubst_value sigmavalue tauvalue thetavalue Eqvalue s0) (compSubstSubst_comp (up_value_value sigmavalue) (up_value_value tauvalue) (up_value_value thetavalue) (up_subst_subst_value_value (_) (_) (_) Eqvalue) s1) (compSubstSubst_comp (up_value_value sigmavalue) (up_value_value tauvalue) (up_value_value thetavalue) (up_subst_subst_value_value (_) (_) (_) Eqvalue) s2)
-    | caseP (_) s0 s1 => congr_caseP (compSubstSubst_value sigmavalue tauvalue thetavalue Eqvalue s0) (compSubstSubst_comp (up_value_value (up_value_value sigmavalue)) (up_value_value (up_value_value tauvalue)) (up_value_value (up_value_value thetavalue)) (up_subst_subst_value_value (_) (_) (_) (up_subst_subst_value_value (_) (_) (_) Eqvalue)) s1)
+    | force (_) s0 => congr_force ((compSubstSubst_value sigmavalue tauvalue thetavalue Eqvalue) s0)
+    | lambda (_) s0 => congr_lambda ((compSubstSubst_comp (up_value_value sigmavalue) (up_value_value tauvalue) (up_value_value thetavalue) (up_subst_subst_value_value (_) (_) (_) Eqvalue)) s0)
+    | app (_) s0 s1 => congr_app ((compSubstSubst_comp sigmavalue tauvalue thetavalue Eqvalue) s0) ((compSubstSubst_value sigmavalue tauvalue thetavalue Eqvalue) s1)
+    | tuple (_) s0 s1 => congr_tuple ((compSubstSubst_comp sigmavalue tauvalue thetavalue Eqvalue) s0) ((compSubstSubst_comp sigmavalue tauvalue thetavalue Eqvalue) s1)
+    | ret (_) s0 => congr_ret ((compSubstSubst_value sigmavalue tauvalue thetavalue Eqvalue) s0)
+    | letin (_) s0 s1 => congr_letin ((compSubstSubst_comp sigmavalue tauvalue thetavalue Eqvalue) s0) ((compSubstSubst_comp (up_value_value sigmavalue) (up_value_value tauvalue) (up_value_value thetavalue) (up_subst_subst_value_value (_) (_) (_) Eqvalue)) s1)
+    | proj (_) s0 s1 => congr_proj ((fun x => (eq_refl) x) s0) ((compSubstSubst_comp sigmavalue tauvalue thetavalue Eqvalue) s1)
+    | caseZ (_) s0 => congr_caseZ ((compSubstSubst_value sigmavalue tauvalue thetavalue Eqvalue) s0)
+    | caseS (_) s0 s1 s2 => congr_caseS ((compSubstSubst_value sigmavalue tauvalue thetavalue Eqvalue) s0) ((compSubstSubst_comp (up_value_value sigmavalue) (up_value_value tauvalue) (up_value_value thetavalue) (up_subst_subst_value_value (_) (_) (_) Eqvalue)) s1) ((compSubstSubst_comp (up_value_value sigmavalue) (up_value_value tauvalue) (up_value_value thetavalue) (up_subst_subst_value_value (_) (_) (_) Eqvalue)) s2)
+    | caseP (_) s0 s1 => congr_caseP ((compSubstSubst_value sigmavalue tauvalue thetavalue Eqvalue) s0) ((compSubstSubst_comp (up_value_value (up_value_value sigmavalue)) (up_value_value (up_value_value tauvalue)) (up_value_value (up_value_value thetavalue)) (up_subst_subst_value_value (_) (_) (_) (up_subst_subst_value_value (_) (_) (_) Eqvalue))) s1)
     end.
 
-Definition rinstInst_up_value_value { m : nat } { nvalue : nat } (xi : fin (m) -> fin (nvalue)) (sigma : fin (m) -> value (nvalue)) (Eq : forall x, (funcomp (var_value (nvalue)) xi) x = sigma x) : forall x, (funcomp (var_value (S nvalue)) (upRen_value_value xi)) x = (up_value_value sigma) x :=
+Definition rinstInst_up_value_value { m : nat } { nvalue : nat } (xi : (fin) (m) -> (fin) (nvalue)) (sigma : (fin) (m) -> value (nvalue)) (Eq : forall x, ((funcomp) (var_value (nvalue)) xi) x = sigma x) : forall x, ((funcomp) (var_value ((S) nvalue)) (upRen_value_value xi)) x = (up_value_value sigma) x :=
   fun n => match n with
-  | Some n => ap (ren_value shift) (Eq n)
-  | None => eq_refl
+  | Some fin_n => (ap) (ren_value (shift)) (Eq fin_n)
+  | None  => eq_refl
   end.
 
-Fixpoint rinst_inst_value { mvalue : nat } { nvalue : nat } (xivalue : fin (mvalue) -> fin (nvalue)) (sigmavalue : fin (mvalue) -> value (nvalue)) (Eqvalue : forall x, (funcomp (var_value (nvalue)) xivalue) x = sigmavalue x) (s : value (mvalue)) : ren_value xivalue s = subst_value sigmavalue s :=
-    match s with
+Fixpoint rinst_inst_value { mvalue : nat } { nvalue : nat } (xivalue : (fin) (mvalue) -> (fin) (nvalue)) (sigmavalue : (fin) (mvalue) -> value (nvalue)) (Eqvalue : forall x, ((funcomp) (var_value (nvalue)) xivalue) x = sigmavalue x) (s : value (mvalue)) : ren_value xivalue s = subst_value sigmavalue s :=
+    match s return ren_value xivalue s = subst_value sigmavalue s with
     | var_value (_) s => Eqvalue s
     | u (_)  => congr_u 
-    | pair (_) s0 s1 => congr_pair (rinst_inst_value xivalue sigmavalue Eqvalue s0) (rinst_inst_value xivalue sigmavalue Eqvalue s1)
-    | inj (_) s0 s1 => congr_inj (eq_refl s0) (rinst_inst_value xivalue sigmavalue Eqvalue s1)
-    | thunk (_) s0 => congr_thunk (rinst_inst_comp xivalue sigmavalue Eqvalue s0)
+    | pair (_) s0 s1 => congr_pair ((rinst_inst_value xivalue sigmavalue Eqvalue) s0) ((rinst_inst_value xivalue sigmavalue Eqvalue) s1)
+    | inj (_) s0 s1 => congr_inj ((fun x => (eq_refl) x) s0) ((rinst_inst_value xivalue sigmavalue Eqvalue) s1)
+    | thunk (_) s0 => congr_thunk ((rinst_inst_comp xivalue sigmavalue Eqvalue) s0)
     end
- with rinst_inst_comp { mvalue : nat } { nvalue : nat } (xivalue : fin (mvalue) -> fin (nvalue)) (sigmavalue : fin (mvalue) -> value (nvalue)) (Eqvalue : forall x, (funcomp (var_value (nvalue)) xivalue) x = sigmavalue x) (s : comp (mvalue)) : ren_comp xivalue s = subst_comp sigmavalue s :=
-    match s with
+ with rinst_inst_comp { mvalue : nat } { nvalue : nat } (xivalue : (fin) (mvalue) -> (fin) (nvalue)) (sigmavalue : (fin) (mvalue) -> value (nvalue)) (Eqvalue : forall x, ((funcomp) (var_value (nvalue)) xivalue) x = sigmavalue x) (s : comp (mvalue)) : ren_comp xivalue s = subst_comp sigmavalue s :=
+    match s return ren_comp xivalue s = subst_comp sigmavalue s with
     | cu (_)  => congr_cu 
-    | force (_) s0 => congr_force (rinst_inst_value xivalue sigmavalue Eqvalue s0)
-    | lambda (_) s0 => congr_lambda (rinst_inst_comp (upRen_value_value xivalue) (up_value_value sigmavalue) (rinstInst_up_value_value (_) (_) Eqvalue) s0)
-    | app (_) s0 s1 => congr_app (rinst_inst_comp xivalue sigmavalue Eqvalue s0) (rinst_inst_value xivalue sigmavalue Eqvalue s1)
-    | tuple (_) s0 s1 => congr_tuple (rinst_inst_comp xivalue sigmavalue Eqvalue s0) (rinst_inst_comp xivalue sigmavalue Eqvalue s1)
-    | ret (_) s0 => congr_ret (rinst_inst_value xivalue sigmavalue Eqvalue s0)
-    | letin (_) s0 s1 => congr_letin (rinst_inst_comp xivalue sigmavalue Eqvalue s0) (rinst_inst_comp (upRen_value_value xivalue) (up_value_value sigmavalue) (rinstInst_up_value_value (_) (_) Eqvalue) s1)
-    | proj (_) s0 s1 => congr_proj (eq_refl s0) (rinst_inst_comp xivalue sigmavalue Eqvalue s1)
-    | caseZ (_) s0 => congr_caseZ (rinst_inst_value xivalue sigmavalue Eqvalue s0)
-    | caseS (_) s0 s1 s2 => congr_caseS (rinst_inst_value xivalue sigmavalue Eqvalue s0) (rinst_inst_comp (upRen_value_value xivalue) (up_value_value sigmavalue) (rinstInst_up_value_value (_) (_) Eqvalue) s1) (rinst_inst_comp (upRen_value_value xivalue) (up_value_value sigmavalue) (rinstInst_up_value_value (_) (_) Eqvalue) s2)
-    | caseP (_) s0 s1 => congr_caseP (rinst_inst_value xivalue sigmavalue Eqvalue s0) (rinst_inst_comp (upRen_value_value (upRen_value_value xivalue)) (up_value_value (up_value_value sigmavalue)) (rinstInst_up_value_value (_) (_) (rinstInst_up_value_value (_) (_) Eqvalue)) s1)
+    | force (_) s0 => congr_force ((rinst_inst_value xivalue sigmavalue Eqvalue) s0)
+    | lambda (_) s0 => congr_lambda ((rinst_inst_comp (upRen_value_value xivalue) (up_value_value sigmavalue) (rinstInst_up_value_value (_) (_) Eqvalue)) s0)
+    | app (_) s0 s1 => congr_app ((rinst_inst_comp xivalue sigmavalue Eqvalue) s0) ((rinst_inst_value xivalue sigmavalue Eqvalue) s1)
+    | tuple (_) s0 s1 => congr_tuple ((rinst_inst_comp xivalue sigmavalue Eqvalue) s0) ((rinst_inst_comp xivalue sigmavalue Eqvalue) s1)
+    | ret (_) s0 => congr_ret ((rinst_inst_value xivalue sigmavalue Eqvalue) s0)
+    | letin (_) s0 s1 => congr_letin ((rinst_inst_comp xivalue sigmavalue Eqvalue) s0) ((rinst_inst_comp (upRen_value_value xivalue) (up_value_value sigmavalue) (rinstInst_up_value_value (_) (_) Eqvalue)) s1)
+    | proj (_) s0 s1 => congr_proj ((fun x => (eq_refl) x) s0) ((rinst_inst_comp xivalue sigmavalue Eqvalue) s1)
+    | caseZ (_) s0 => congr_caseZ ((rinst_inst_value xivalue sigmavalue Eqvalue) s0)
+    | caseS (_) s0 s1 s2 => congr_caseS ((rinst_inst_value xivalue sigmavalue Eqvalue) s0) ((rinst_inst_comp (upRen_value_value xivalue) (up_value_value sigmavalue) (rinstInst_up_value_value (_) (_) Eqvalue)) s1) ((rinst_inst_comp (upRen_value_value xivalue) (up_value_value sigmavalue) (rinstInst_up_value_value (_) (_) Eqvalue)) s2)
+    | caseP (_) s0 s1 => congr_caseP ((rinst_inst_value xivalue sigmavalue Eqvalue) s0) ((rinst_inst_comp (upRen_value_value (upRen_value_value xivalue)) (up_value_value (up_value_value sigmavalue)) (rinstInst_up_value_value (_) (_) (rinstInst_up_value_value (_) (_) Eqvalue))) s1)
     end.
+
+Lemma rinstInst_value { mvalue : nat } { nvalue : nat } (xivalue : (fin) (mvalue) -> (fin) (nvalue)) : ren_value xivalue = subst_value ((funcomp) (var_value (nvalue)) xivalue) .
+Proof. exact ((FunctionalExtensionality.functional_extensionality _ _ ) (fun x => rinst_inst_value xivalue (_) (fun n => eq_refl) x)). Qed.
+
+Lemma rinstInst_comp { mvalue : nat } { nvalue : nat } (xivalue : (fin) (mvalue) -> (fin) (nvalue)) : ren_comp xivalue = subst_comp ((funcomp) (var_value (nvalue)) xivalue) .
+Proof. exact ((FunctionalExtensionality.functional_extensionality _ _ ) (fun x => rinst_inst_comp xivalue (_) (fun n => eq_refl) x)). Qed.
 
 Lemma instId_value { mvalue : nat } : subst_value (var_value (mvalue)) = id .
-Proof. exact (FunctionalExtensionality.functional_extensionality _ _ (fun x => idSubst_value (var_value (mvalue)) (fun n => eq_refl) (id x))). Qed.
+Proof. exact ((FunctionalExtensionality.functional_extensionality _ _ ) (fun x => idSubst_value (var_value (mvalue)) (fun n => eq_refl) ((id) x))). Qed.
 
 Lemma instId_comp { mvalue : nat } : subst_comp (var_value (mvalue)) = id .
-Proof. exact (FunctionalExtensionality.functional_extensionality _ _ (fun x => idSubst_comp (var_value (mvalue)) (fun n => eq_refl) (id x))). Qed.
+Proof. exact ((FunctionalExtensionality.functional_extensionality _ _ ) (fun x => idSubst_comp (var_value (mvalue)) (fun n => eq_refl) ((id) x))). Qed.
 
-Lemma varL_value { mvalue : nat } { nvalue : nat } (sigmavalue : fin (mvalue) -> value (nvalue)) : funcomp (subst_value sigmavalue) (var_value (mvalue)) = sigmavalue .
-Proof. exact (FunctionalExtensionality.functional_extensionality _ _ (fun x => eq_refl)). Qed.
+Lemma rinstId_value { mvalue : nat } : @ren_value (mvalue) (mvalue) (id) = id .
+Proof. exact ((eq_trans) (rinstInst_value ((id) (_))) instId_value). Qed.
 
-Lemma varLRen_value { mvalue : nat } { nvalue : nat } (xivalue : fin (mvalue) -> fin (nvalue)) : funcomp (ren_value xivalue) (var_value (mvalue)) = funcomp (var_value (nvalue)) xivalue .
-Proof. exact (FunctionalExtensionality.functional_extensionality _ _ (fun x => eq_refl)). Qed.
+Lemma rinstId_comp { mvalue : nat } : @ren_comp (mvalue) (mvalue) (id) = id .
+Proof. exact ((eq_trans) (rinstInst_comp ((id) (_))) instId_comp). Qed.
 
-Lemma rinstInst_value { mvalue : nat } { nvalue : nat } (xivalue : fin (mvalue) -> fin (nvalue)) : ren_value xivalue = subst_value (funcomp (var_value (nvalue)) xivalue) .
-Proof. exact (FunctionalExtensionality.functional_extensionality _ _ (fun x => rinst_inst_value xivalue (_) (fun n => eq_refl) x)). Qed.
+Lemma varL_value { mvalue : nat } { nvalue : nat } (sigmavalue : (fin) (mvalue) -> value (nvalue)) : (funcomp) (subst_value sigmavalue) (var_value (mvalue)) = sigmavalue .
+Proof. exact ((FunctionalExtensionality.functional_extensionality _ _ ) (fun x => eq_refl)). Qed.
 
-Lemma rinstInst_comp { mvalue : nat } { nvalue : nat } (xivalue : fin (mvalue) -> fin (nvalue)) : ren_comp xivalue = subst_comp (funcomp (var_value (nvalue)) xivalue) .
-Proof. exact (FunctionalExtensionality.functional_extensionality _ _ (fun x => rinst_inst_comp xivalue (_) (fun n => eq_refl) x)). Qed.
+Lemma varLRen_value { mvalue : nat } { nvalue : nat } (xivalue : (fin) (mvalue) -> (fin) (nvalue)) : (funcomp) (ren_value xivalue) (var_value (mvalue)) = (funcomp) (var_value (nvalue)) xivalue .
+Proof. exact ((FunctionalExtensionality.functional_extensionality _ _ ) (fun x => eq_refl)). Qed.
 
-Lemma compComp_value { kvalue : nat } { lvalue : nat } { mvalue : nat } (sigmavalue : fin (mvalue) -> value (kvalue)) (tauvalue : fin (kvalue) -> value (lvalue)) (s : value (mvalue)) : subst_value tauvalue (subst_value sigmavalue s) = subst_value (funcomp (subst_value tauvalue) sigmavalue) s .
+Lemma compComp_value { kvalue : nat } { lvalue : nat } { mvalue : nat } (sigmavalue : (fin) (mvalue) -> value (kvalue)) (tauvalue : (fin) (kvalue) -> value (lvalue)) (s : value (mvalue)) : subst_value tauvalue (subst_value sigmavalue s) = subst_value ((funcomp) (subst_value tauvalue) sigmavalue) s .
 Proof. exact (compSubstSubst_value sigmavalue tauvalue (_) (fun n => eq_refl) s). Qed.
 
-Lemma compComp_comp { kvalue : nat } { lvalue : nat } { mvalue : nat } (sigmavalue : fin (mvalue) -> value (kvalue)) (tauvalue : fin (kvalue) -> value (lvalue)) (s : comp (mvalue)) : subst_comp tauvalue (subst_comp sigmavalue s) = subst_comp (funcomp (subst_value tauvalue) sigmavalue) s .
+Lemma compComp_comp { kvalue : nat } { lvalue : nat } { mvalue : nat } (sigmavalue : (fin) (mvalue) -> value (kvalue)) (tauvalue : (fin) (kvalue) -> value (lvalue)) (s : comp (mvalue)) : subst_comp tauvalue (subst_comp sigmavalue s) = subst_comp ((funcomp) (subst_value tauvalue) sigmavalue) s .
 Proof. exact (compSubstSubst_comp sigmavalue tauvalue (_) (fun n => eq_refl) s). Qed.
 
-Lemma compComp'_value { kvalue : nat } { lvalue : nat } { mvalue : nat } (sigmavalue : fin (mvalue) -> value (kvalue)) (tauvalue : fin (kvalue) -> value (lvalue)) : funcomp (subst_value tauvalue) (subst_value sigmavalue) = subst_value (funcomp (subst_value tauvalue) sigmavalue) .
-Proof. exact (FunctionalExtensionality.functional_extensionality _ _ (fun n => compComp_value sigmavalue tauvalue n)). Qed.
+Lemma compComp'_value { kvalue : nat } { lvalue : nat } { mvalue : nat } (sigmavalue : (fin) (mvalue) -> value (kvalue)) (tauvalue : (fin) (kvalue) -> value (lvalue)) : (funcomp) (subst_value tauvalue) (subst_value sigmavalue) = subst_value ((funcomp) (subst_value tauvalue) sigmavalue) .
+Proof. exact ((FunctionalExtensionality.functional_extensionality _ _ ) (fun n => compComp_value sigmavalue tauvalue n)). Qed.
 
-Lemma compComp'_comp { kvalue : nat } { lvalue : nat } { mvalue : nat } (sigmavalue : fin (mvalue) -> value (kvalue)) (tauvalue : fin (kvalue) -> value (lvalue)) : funcomp (subst_comp tauvalue) (subst_comp sigmavalue) = subst_comp (funcomp (subst_value tauvalue) sigmavalue) .
-Proof. exact (FunctionalExtensionality.functional_extensionality _ _ (fun n => compComp_comp sigmavalue tauvalue n)). Qed.
+Lemma compComp'_comp { kvalue : nat } { lvalue : nat } { mvalue : nat } (sigmavalue : (fin) (mvalue) -> value (kvalue)) (tauvalue : (fin) (kvalue) -> value (lvalue)) : (funcomp) (subst_comp tauvalue) (subst_comp sigmavalue) = subst_comp ((funcomp) (subst_value tauvalue) sigmavalue) .
+Proof. exact ((FunctionalExtensionality.functional_extensionality _ _ ) (fun n => compComp_comp sigmavalue tauvalue n)). Qed.
 
-Lemma compRen_value { kvalue : nat } { lvalue : nat } { mvalue : nat } (sigmavalue : fin (mvalue) -> value (kvalue)) (zetavalue : fin (kvalue) -> fin (lvalue)) (s : value (mvalue)) : ren_value zetavalue (subst_value sigmavalue s) = subst_value (funcomp (ren_value zetavalue) sigmavalue) s .
-Proof. exact (compSubstRen__value sigmavalue zetavalue (_) (fun n => eq_refl) s). Qed.
+Lemma compRen_value { kvalue : nat } { lvalue : nat } { mvalue : nat } (sigmavalue : (fin) (mvalue) -> value (kvalue)) (zetavalue : (fin) (kvalue) -> (fin) (lvalue)) (s : value (mvalue)) : ren_value zetavalue (subst_value sigmavalue s) = subst_value ((funcomp) (ren_value zetavalue) sigmavalue) s .
+Proof. exact (compSubstRen_value sigmavalue zetavalue (_) (fun n => eq_refl) s). Qed.
 
-Lemma compRen_comp { kvalue : nat } { lvalue : nat } { mvalue : nat } (sigmavalue : fin (mvalue) -> value (kvalue)) (zetavalue : fin (kvalue) -> fin (lvalue)) (s : comp (mvalue)) : ren_comp zetavalue (subst_comp sigmavalue s) = subst_comp (funcomp (ren_value zetavalue) sigmavalue) s .
-Proof. exact (compSubstRen__comp sigmavalue zetavalue (_) (fun n => eq_refl) s). Qed.
+Lemma compRen_comp { kvalue : nat } { lvalue : nat } { mvalue : nat } (sigmavalue : (fin) (mvalue) -> value (kvalue)) (zetavalue : (fin) (kvalue) -> (fin) (lvalue)) (s : comp (mvalue)) : ren_comp zetavalue (subst_comp sigmavalue s) = subst_comp ((funcomp) (ren_value zetavalue) sigmavalue) s .
+Proof. exact (compSubstRen_comp sigmavalue zetavalue (_) (fun n => eq_refl) s). Qed.
 
-Lemma compRen'_value { kvalue : nat } { lvalue : nat } { mvalue : nat } (sigmavalue : fin (mvalue) -> value (kvalue)) (zetavalue : fin (kvalue) -> fin (lvalue)) : funcomp (ren_value zetavalue) (subst_value sigmavalue) = subst_value (funcomp (ren_value zetavalue) sigmavalue) .
-Proof. exact (FunctionalExtensionality.functional_extensionality _ _ (fun n => compRen_value sigmavalue zetavalue n)). Qed.
+Lemma compRen'_value { kvalue : nat } { lvalue : nat } { mvalue : nat } (sigmavalue : (fin) (mvalue) -> value (kvalue)) (zetavalue : (fin) (kvalue) -> (fin) (lvalue)) : (funcomp) (ren_value zetavalue) (subst_value sigmavalue) = subst_value ((funcomp) (ren_value zetavalue) sigmavalue) .
+Proof. exact ((FunctionalExtensionality.functional_extensionality _ _ ) (fun n => compRen_value sigmavalue zetavalue n)). Qed.
 
-Lemma compRen'_comp { kvalue : nat } { lvalue : nat } { mvalue : nat } (sigmavalue : fin (mvalue) -> value (kvalue)) (zetavalue : fin (kvalue) -> fin (lvalue)) : funcomp (ren_comp zetavalue) (subst_comp sigmavalue) = subst_comp (funcomp (ren_value zetavalue) sigmavalue) .
-Proof. exact (FunctionalExtensionality.functional_extensionality _ _ (fun n => compRen_comp sigmavalue zetavalue n)). Qed.
+Lemma compRen'_comp { kvalue : nat } { lvalue : nat } { mvalue : nat } (sigmavalue : (fin) (mvalue) -> value (kvalue)) (zetavalue : (fin) (kvalue) -> (fin) (lvalue)) : (funcomp) (ren_comp zetavalue) (subst_comp sigmavalue) = subst_comp ((funcomp) (ren_value zetavalue) sigmavalue) .
+Proof. exact ((FunctionalExtensionality.functional_extensionality _ _ ) (fun n => compRen_comp sigmavalue zetavalue n)). Qed.
 
-Lemma renComp_value { kvalue : nat } { lvalue : nat } { mvalue : nat } (xivalue : fin (mvalue) -> fin (kvalue)) (tauvalue : fin (kvalue) -> value (lvalue)) (s : value (mvalue)) : subst_value tauvalue (ren_value xivalue s) = subst_value (funcomp tauvalue xivalue) s .
+Lemma renComp_value { kvalue : nat } { lvalue : nat } { mvalue : nat } (xivalue : (fin) (mvalue) -> (fin) (kvalue)) (tauvalue : (fin) (kvalue) -> value (lvalue)) (s : value (mvalue)) : subst_value tauvalue (ren_value xivalue s) = subst_value ((funcomp) tauvalue xivalue) s .
 Proof. exact (compRenSubst_value xivalue tauvalue (_) (fun n => eq_refl) s). Qed.
 
-Lemma renComp_comp { kvalue : nat } { lvalue : nat } { mvalue : nat } (xivalue : fin (mvalue) -> fin (kvalue)) (tauvalue : fin (kvalue) -> value (lvalue)) (s : comp (mvalue)) : subst_comp tauvalue (ren_comp xivalue s) = subst_comp (funcomp tauvalue xivalue) s .
+Lemma renComp_comp { kvalue : nat } { lvalue : nat } { mvalue : nat } (xivalue : (fin) (mvalue) -> (fin) (kvalue)) (tauvalue : (fin) (kvalue) -> value (lvalue)) (s : comp (mvalue)) : subst_comp tauvalue (ren_comp xivalue s) = subst_comp ((funcomp) tauvalue xivalue) s .
 Proof. exact (compRenSubst_comp xivalue tauvalue (_) (fun n => eq_refl) s). Qed.
 
-Lemma renComp'_value { kvalue : nat } { lvalue : nat } { mvalue : nat } (xivalue : fin (mvalue) -> fin (kvalue)) (tauvalue : fin (kvalue) -> value (lvalue)) : funcomp (subst_value tauvalue) (ren_value xivalue) = subst_value (funcomp tauvalue xivalue) .
-Proof. exact (FunctionalExtensionality.functional_extensionality _ _ (fun n => renComp_value xivalue tauvalue n)). Qed.
+Lemma renComp'_value { kvalue : nat } { lvalue : nat } { mvalue : nat } (xivalue : (fin) (mvalue) -> (fin) (kvalue)) (tauvalue : (fin) (kvalue) -> value (lvalue)) : (funcomp) (subst_value tauvalue) (ren_value xivalue) = subst_value ((funcomp) tauvalue xivalue) .
+Proof. exact ((FunctionalExtensionality.functional_extensionality _ _ ) (fun n => renComp_value xivalue tauvalue n)). Qed.
 
-Lemma renComp'_comp { kvalue : nat } { lvalue : nat } { mvalue : nat } (xivalue : fin (mvalue) -> fin (kvalue)) (tauvalue : fin (kvalue) -> value (lvalue)) : funcomp (subst_comp tauvalue) (ren_comp xivalue) = subst_comp (funcomp tauvalue xivalue) .
-Proof. exact (FunctionalExtensionality.functional_extensionality _ _ (fun n => renComp_comp xivalue tauvalue n)). Qed.
+Lemma renComp'_comp { kvalue : nat } { lvalue : nat } { mvalue : nat } (xivalue : (fin) (mvalue) -> (fin) (kvalue)) (tauvalue : (fin) (kvalue) -> value (lvalue)) : (funcomp) (subst_comp tauvalue) (ren_comp xivalue) = subst_comp ((funcomp) tauvalue xivalue) .
+Proof. exact ((FunctionalExtensionality.functional_extensionality _ _ ) (fun n => renComp_comp xivalue tauvalue n)). Qed.
 
-Lemma renRen_value { kvalue : nat } { lvalue : nat } { mvalue : nat } (xivalue : fin (mvalue) -> fin (kvalue)) (zetavalue : fin (kvalue) -> fin (lvalue)) (s : value (mvalue)) : ren_value zetavalue (ren_value xivalue s) = ren_value (funcomp zetavalue xivalue) s .
+Lemma renRen_value { kvalue : nat } { lvalue : nat } { mvalue : nat } (xivalue : (fin) (mvalue) -> (fin) (kvalue)) (zetavalue : (fin) (kvalue) -> (fin) (lvalue)) (s : value (mvalue)) : ren_value zetavalue (ren_value xivalue s) = ren_value ((funcomp) zetavalue xivalue) s .
 Proof. exact (compRenRen_value xivalue zetavalue (_) (fun n => eq_refl) s). Qed.
 
-Lemma renRen_comp { kvalue : nat } { lvalue : nat } { mvalue : nat } (xivalue : fin (mvalue) -> fin (kvalue)) (zetavalue : fin (kvalue) -> fin (lvalue)) (s : comp (mvalue)) : ren_comp zetavalue (ren_comp xivalue s) = ren_comp (funcomp zetavalue xivalue) s .
+Lemma renRen_comp { kvalue : nat } { lvalue : nat } { mvalue : nat } (xivalue : (fin) (mvalue) -> (fin) (kvalue)) (zetavalue : (fin) (kvalue) -> (fin) (lvalue)) (s : comp (mvalue)) : ren_comp zetavalue (ren_comp xivalue s) = ren_comp ((funcomp) zetavalue xivalue) s .
 Proof. exact (compRenRen_comp xivalue zetavalue (_) (fun n => eq_refl) s). Qed.
 
-Lemma renRen'_value { kvalue : nat } { lvalue : nat } { mvalue : nat } (xivalue : fin (mvalue) -> fin (kvalue)) (zetavalue : fin (kvalue) -> fin (lvalue)) : funcomp (ren_value zetavalue) (ren_value xivalue) = ren_value (funcomp zetavalue xivalue) .
-Proof. exact (FunctionalExtensionality.functional_extensionality _ _ (fun n => renRen_value xivalue zetavalue n)). Qed.
+Lemma renRen'_value { kvalue : nat } { lvalue : nat } { mvalue : nat } (xivalue : (fin) (mvalue) -> (fin) (kvalue)) (zetavalue : (fin) (kvalue) -> (fin) (lvalue)) : (funcomp) (ren_value zetavalue) (ren_value xivalue) = ren_value ((funcomp) zetavalue xivalue) .
+Proof. exact ((FunctionalExtensionality.functional_extensionality _ _ ) (fun n => renRen_value xivalue zetavalue n)). Qed.
 
-Lemma renRen'_comp { kvalue : nat } { lvalue : nat } { mvalue : nat } (xivalue : fin (mvalue) -> fin (kvalue)) (zetavalue : fin (kvalue) -> fin (lvalue)) : funcomp (ren_comp zetavalue) (ren_comp xivalue) = ren_comp (funcomp zetavalue xivalue) .
-Proof. exact (FunctionalExtensionality.functional_extensionality _ _ (fun n => renRen_comp xivalue zetavalue n)). Qed.
+Lemma renRen'_comp { kvalue : nat } { lvalue : nat } { mvalue : nat } (xivalue : (fin) (mvalue) -> (fin) (kvalue)) (zetavalue : (fin) (kvalue) -> (fin) (lvalue)) : (funcomp) (ren_comp zetavalue) (ren_comp xivalue) = ren_comp ((funcomp) zetavalue xivalue) .
+Proof. exact ((FunctionalExtensionality.functional_extensionality _ _ ) (fun n => renRen_comp xivalue zetavalue n)). Qed.
+
+End valuecomp.
 
 Arguments var_value {nvalue}.
 
@@ -479,38 +497,61 @@ Arguments caseS {nvalue}.
 
 Arguments caseP {nvalue}.
 
-Instance Subst_value : Subst1 value value := @subst_value .
+Global Instance Subst_value { mvalue : nat } { nvalue : nat } : Subst1 ((fin) (mvalue) -> value (nvalue)) (value (mvalue)) (value (nvalue)) := @subst_value (mvalue) (nvalue) .
 
-Instance Subst_comp : Subst1 value comp := @subst_comp .
+Global Instance Subst_comp { mvalue : nat } { nvalue : nat } : Subst1 ((fin) (mvalue) -> value (nvalue)) (comp (mvalue)) (comp (nvalue)) := @subst_comp (mvalue) (nvalue) .
 
-Instance Ren_value : Ren1 value := @ren_value .
+Global Instance Ren_value { mvalue : nat } { nvalue : nat } : Ren1 ((fin) (mvalue) -> (fin) (nvalue)) (value (mvalue)) (value (nvalue)) := @ren_value (mvalue) (nvalue) .
 
-Instance Ren_comp : Ren1 comp := @ren_comp .
+Global Instance Ren_comp { mvalue : nat } { nvalue : nat } : Ren1 ((fin) (mvalue) -> (fin) (nvalue)) (comp (mvalue)) (comp (nvalue)) := @ren_comp (mvalue) (nvalue) .
 
-Instance VarInstance_value : Var value := @var_value .
+Global Instance VarInstance_value { mvalue : nat } : Var ((fin) (mvalue)) (value (mvalue)) := @var_value (mvalue) .
 
-Notation "x '__value'" := (@ids value VarInstance_value (_) x) (at level 30, format "x __value") : subst_scope.
+Notation "x '__value'" := (var_value x) (at level 5, format "x __value") : subst_scope.
 
-Notation "⇑__value" := (@up_value_value (_)) (only printing) : subst_scope.
+Notation "x '__value'" := (@ids (_) (_) VarInstance_value x) (at level 5, only printing, format "x __value") : subst_scope.
 
-Ltac auto_unfold := repeat unfold subst1,  ren1,  subst2,  ren2,  Subst1,  Ren1,  Subst2,  Ren2,  ids,  Subst_value,  Subst_comp,  Ren_value,  Ren_comp,  VarInstance_value.
+Notation "'var'" := (var_value) (only printing, at level 1) : subst_scope.
 
-Ltac auto_fold := try fold VarInstance_value;  try fold (@ids _ VarInstance_value);  try fold Subst_value;  try fold Subst_comp;  try fold (@subst1 _ _ Subst_value);  try fold (@subst1 _ _ Subst_comp);  try fold Ren_value;  try fold Ren_comp;  try fold (@ren1 _ Ren_value);  try fold (@ren1 _ Ren_comp).
+Class Up_value X Y := up_value : X -> Y.
 
-Tactic Notation "auto_unfold" "in" "*" := repeat unfold subst1,  ren1,  subst2,  ren2,  Subst1,  Ren1,  Subst2,  Ren2,  ids,  Subst_value,  Subst_comp,  Ren_value,  Ren_comp,  VarInstance_value in *.
+Notation "↑__value" := (up_value) (only printing) : subst_scope.
 
-Tactic Notation "auto_fold" "in" "*" := try fold VarInstance_value in *;  try fold (@ids _ VarInstance_value) in *;  try fold Subst_value in *;  try fold Subst_comp in *;  try fold (@subst1 _ _ Subst_value) in *;  try fold (@subst1 _ _ Subst_comp) in *;  try fold Ren_value in *;  try fold Ren_comp in *;  try fold (@ren1 _ Ren_value) in *;  try fold (@ren1 _ Ren_comp) in *.
+Notation "↑__value" := (up_value_value) (only printing) : subst_scope.
 
-Ltac asimpl' := repeat first [progress rewrite ?instId_value| progress rewrite ?compComp_value| progress rewrite ?compComp'_value| progress rewrite ?compRen_value| progress rewrite ?compRen'_value| progress rewrite ?renComp_value| progress rewrite ?renComp'_value| progress rewrite ?renRen_value| progress rewrite ?renRen'_value| progress rewrite ?instId_comp| progress rewrite ?compComp_comp| progress rewrite ?compComp'_comp| progress rewrite ?compRen_comp| progress rewrite ?compRen'_comp| progress rewrite ?renComp_comp| progress rewrite ?renComp'_comp| progress rewrite ?renRen_comp| progress rewrite ?renRen'_comp| progress rewrite ?varL_value| progress rewrite ?varLRen_value| progress (unfold up_ren, upRen_value_value, up_value_value)| progress (cbn [subst_value subst_comp ren_value ren_comp])| fsimpl].
+Global Instance Up_value_value { m : nat } { nvalue : nat } : Up_value (_) (_) := @up_value_value (m) (nvalue) .
 
-Ltac asimpl := auto_unfold; asimpl'; auto_fold.
+Notation "s [ sigmavalue ]" := (subst_value sigmavalue s) (at level 7, left associativity, only printing) : subst_scope.
+
+Notation "[ sigmavalue ]" := (subst_value sigmavalue) (at level 1, left associativity, only printing) : fscope.
+
+Notation "s ⟨ xivalue ⟩" := (ren_value xivalue s) (at level 7, left associativity, only printing) : subst_scope.
+
+Notation "⟨ xivalue ⟩" := (ren_value xivalue) (at level 1, left associativity, only printing) : fscope.
+
+Notation "s [ sigmavalue ]" := (subst_comp sigmavalue s) (at level 7, left associativity, only printing) : subst_scope.
+
+Notation "[ sigmavalue ]" := (subst_comp sigmavalue) (at level 1, left associativity, only printing) : fscope.
+
+Notation "s ⟨ xivalue ⟩" := (ren_comp xivalue s) (at level 7, left associativity, only printing) : subst_scope.
+
+Notation "⟨ xivalue ⟩" := (ren_comp xivalue) (at level 1, left associativity, only printing) : fscope.
+
+Ltac auto_unfold := repeat unfold subst1,  subst2,  Subst1,  Subst2,  ids,  ren1,  ren2,  Ren1,  Ren2,  Subst_value,  Subst_comp,  Ren_value,  Ren_comp,  VarInstance_value.
+
+Tactic Notation "auto_unfold" "in" "*" := repeat unfold subst1,  subst2,  Subst1,  Subst2,  ids,  ren1,  ren2,  Ren1,  Ren2,  Subst_value,  Subst_comp,  Ren_value,  Ren_comp,  VarInstance_value in *.
+
+Ltac asimpl' := repeat first [progress rewrite ?instId_value| progress rewrite ?compComp_value| progress rewrite ?compComp'_value| progress rewrite ?instId_comp| progress rewrite ?compComp_comp| progress rewrite ?compComp'_comp| progress rewrite ?rinstId_value| progress rewrite ?compRen_value| progress rewrite ?compRen'_value| progress rewrite ?renComp_value| progress rewrite ?renComp'_value| progress rewrite ?renRen_value| progress rewrite ?renRen'_value| progress rewrite ?rinstId_comp| progress rewrite ?compRen_comp| progress rewrite ?compRen'_comp| progress rewrite ?renComp_comp| progress rewrite ?renComp'_comp| progress rewrite ?renRen_comp| progress rewrite ?renRen'_comp| progress rewrite ?varL_value| progress rewrite ?varLRen_value| progress (unfold up_ren, upRen_value_value, up_value_value)| progress (cbn [subst_value subst_comp ren_value ren_comp])| fsimpl].
+
+Ltac asimpl := repeat try unfold_funcomp; auto_unfold in *; asimpl'; repeat try unfold_funcomp.
 
 Tactic Notation "asimpl" "in" hyp(J) := revert J; asimpl; intros J.
 
 Tactic Notation "auto_case" := auto_case (asimpl; cbn; eauto).
 
-Tactic Notation "asimpl" "in" "*" := auto_unfold in *; repeat first [progress rewrite ?instId_value in *| progress rewrite ?compComp_value in *| progress rewrite ?compComp'_value in *| progress rewrite ?compRen_value in *| progress rewrite ?compRen'_value in *| progress rewrite ?renComp_value in *| progress rewrite ?renComp'_value in *| progress rewrite ?renRen_value in *| progress rewrite ?renRen'_value in *| progress rewrite ?instId_comp in *| progress rewrite ?compComp_comp in *| progress rewrite ?compComp'_comp in *| progress rewrite ?compRen_comp in *| progress rewrite ?compRen'_comp in *| progress rewrite ?renComp_comp in *| progress rewrite ?renComp'_comp in *| progress rewrite ?renRen_comp in *| progress rewrite ?renRen'_comp in *| progress rewrite ?varL_value in *| progress rewrite ?varLRen_value in *| progress (unfold up_ren, upRen_value_value, up_value_value in *)| progress (cbn [subst_value subst_comp ren_value ren_comp] in *)| fsimpl in *]; auto_fold in *.
+Tactic Notation "asimpl" "in" "*" := auto_unfold in *; repeat first [progress rewrite ?instId_value in *| progress rewrite ?compComp_value in *| progress rewrite ?compComp'_value in *| progress rewrite ?instId_comp in *| progress rewrite ?compComp_comp in *| progress rewrite ?compComp'_comp in *| progress rewrite ?rinstId_value in *| progress rewrite ?compRen_value in *| progress rewrite ?compRen'_value in *| progress rewrite ?renComp_value in *| progress rewrite ?renComp'_value in *| progress rewrite ?renRen_value in *| progress rewrite ?renRen'_value in *| progress rewrite ?rinstId_comp in *| progress rewrite ?compRen_comp in *| progress rewrite ?compRen'_comp in *| progress rewrite ?renComp_comp in *| progress rewrite ?renComp'_comp in *| progress rewrite ?renRen_comp in *| progress rewrite ?renRen'_comp in *| progress rewrite ?varL_value in *| progress rewrite ?varLRen_value in *| progress (unfold up_ren, upRen_value_value, up_value_value in *)| progress (cbn [subst_value subst_comp ren_value ren_comp] in *)| fsimpl in *].
 
-Ltac substify := auto_unfold; try repeat (erewrite rinst_inst_value; [|now intros]); try repeat (erewrite rinst_inst_comp; [|now intros]); auto_fold.
+Ltac substify := auto_unfold; try repeat (erewrite rinstInst_value); try repeat (erewrite rinstInst_comp).
 
-Ltac renamify := auto_unfold; try repeat (erewrite <- rinst_inst_value; [|intros; now asimpl]); try repeat (erewrite <- rinst_inst_comp; [|intros; now asimpl]); auto_fold.
+Ltac renamify := auto_unfold; try repeat (erewrite <- rinstInst_value); try repeat (erewrite <- rinstInst_comp).
+
